Work on porting to new HOL

basis/TextIOProofScript.sml
@@ -34,20 +34,17 @@ val IOFS_def = Define `
 val IOFS_WO_iobuff_def = Define `
   IOFS_WO_iobuff fs = IOx (fs_ffi_part) fs * &wfFS fs`;
 
-Theorem UNIQUE_IOFS:
- !s. VALID_HEAP s ==> !fs1 fs2 H1 H2. (IOFS fs1 * H1) s /\
-                                      (IOFS fs2 * H2) s ==> fs1 = fs2
-Proof
-  rw[IOFS_def,cfHeapsBaseTheory.IOx_def, fs_ffi_part_def,
+Theorem UNIQUE_IOFS
+`!s. VALID_HEAP s ==> !fs1 fs2 H1 H2. (IOFS fs1 * H1) s /\
+                                      (IOFS fs2 * H2) s ==> fs1 = fs2`
+  (rw[IOFS_def,cfHeapsBaseTheory.IOx_def, fs_ffi_part_def,
      GSYM STAR_ASSOC,encode_def] >>
   IMP_RES_TAC FRAME_UNIQUE_IO >>
-  fs[IO_fs_component_equality]
-QED
+  fs[IO_fs_component_equality]);
 
-Theorem IOFS_FFI_part_hprop:
-   FFI_part_hprop (IOFS fs)
-Proof
-  rw [IOFS_def,
+Theorem IOFS_FFI_part_hprop
+  `FFI_part_hprop (IOFS fs)`
+  (rw [IOFS_def,
       cfHeapsBaseTheory.IO_def, cfHeapsBaseTheory.IOx_def,
       fs_ffi_part_def, cfMainTheory.FFI_part_hprop_def,
     set_sepTheory.SEP_CLAUSES,set_sepTheory.SEP_EXISTS_THM,
@@ -55,17 +52,14 @@ Proof
     cfHeapsBaseTheory.cell_def]
   \\ fs[set_sepTheory.one_STAR,STAR_def]
   \\ imp_res_tac SPLIT_SUBSET >> fs[SUBSET_DEF]
-  \\ metis_tac[]
-QED
+  \\ metis_tac[]);
 
-Theorem IOFS_iobuff_HPROP_INJ[hprop_inj]:
- !fs1 fs2. HPROP_INJ (IOFS fs1) (IOFS fs2) (fs2 = fs1)
-Proof
-  rw[HPROP_INJ_def, IOFS_def, GSYM STAR_ASSOC, SEP_CLAUSES, SEP_EXISTS_THM,
+Theorem IOFS_iobuff_HPROP_INJ[hprop_inj]
+`!fs1 fs2. HPROP_INJ (IOFS fs1) (IOFS fs2) (fs2 = fs1)`
+  (rw[HPROP_INJ_def, IOFS_def, GSYM STAR_ASSOC, SEP_CLAUSES, SEP_EXISTS_THM,
      HCOND_EXTRACT] >>
   fs[IOFS_def,cfHeapsBaseTheory.IOx_def, fs_ffi_part_def] >>
-  EQ_TAC >> rpt DISCH_TAC >> IMP_RES_TAC FRAME_UNIQUE_IO >> fs[]
-QED
+  EQ_TAC >> rpt DISCH_TAC >> IMP_RES_TAC FRAME_UNIQUE_IO >> fs[]);
 
 (* "end-user" property *)
 (* abstracts away the lazy list and ensure that standard streams are opened on
@@ -78,35 +72,28 @@ val STDIO_def = Define`
 (* Used by the monadic translator *)
 val MONAD_IO_def = Define `MONAD_IO fs = STDIO fs * &hasFreeFD fs`;
 
-Theorem STDIO_numchars:
-   STDIO (fs with numchars := x) = STDIO fs
-Proof
-  rw[STDIO_def,GSYM STD_streams_numchars]
-QED
+Theorem STDIO_numchars
+  `STDIO (fs with numchars := x) = STDIO fs`
+  (rw[STDIO_def,GSYM STD_streams_numchars]);
 
-Theorem STDIO_bumpFD[simp]:
-   STDIO (bumpFD fd fs n) = STDIO (forwardFD fs fd n)
-Proof
-  rw[bumpFD_forwardFD,STDIO_numchars]
-QED
+Theorem STDIO_bumpFD[simp]
+  `STDIO (bumpFD fd fs n) = STDIO (forwardFD fs fd n)`
+  (rw[bumpFD_forwardFD,STDIO_numchars]);
 
-Theorem UNIQUE_STDIO:
- !s. VALID_HEAP s ==> !fs1 fs2 H1 H2. (STDIO fs1 * H1) s /\
+Theorem UNIQUE_STDIO
+`!s. VALID_HEAP s ==> !fs1 fs2 H1 H2. (STDIO fs1 * H1) s /\
                                       (STDIO fs2 * H2) s ==>
-              (fs1.infds = fs2.infds /\ fs1.inode_tbl = fs2.inode_tbl /\ fs1.maxFD = fs2.maxFD /\ fs1.files = fs2.files)
-Proof
-  rw[STDIO_def,STD_streams_def,SEP_CLAUSES,SEP_EXISTS_THM,STAR_COMM,STAR_ASSOC,cond_STAR] >>
+              (fs1.infds = fs2.infds /\ fs1.files = fs2.files /\ fs1.maxFD = fs2.maxFD)`
+  (rw[STDIO_def,STD_streams_def,SEP_CLAUSES,SEP_EXISTS_THM,STAR_COMM,STAR_ASSOC,cond_STAR] >>
   fs[Once STAR_COMM] >>
   imp_res_tac UNIQUE_IOFS >>
-  cases_on`fs1` >> cases_on`fs2` >> fs[IO_fs_numchars_fupd]
-QED
+  cases_on`fs1` >> cases_on`fs2` >> fs[IO_fs_numchars_fupd]);
 
 (* weak injection theorem *)
-Theorem STDIO_HPROP_INJ[hprop_inj]:
- HPROP_INJ (STDIO fs1) (STDIO fs2)
-           (fs1.infds = fs2.infds /\ fs1.inode_tbl = fs2.inode_tbl /\ fs1.maxFD = fs2.maxFD /\ fs1.files = fs2.files)
-Proof
-  rw[HPROP_INJ_def, GSYM STAR_ASSOC, SEP_CLAUSES, SEP_EXISTS_THM,
+Theorem STDIO_HPROP_INJ[hprop_inj]
+`HPROP_INJ (STDIO fs1) (STDIO fs2)
+           (fs1.infds = fs2.infds /\ fs1.files = fs2.files /\ fs1.maxFD = fs2.maxFD)`
+  (rw[HPROP_INJ_def, GSYM STAR_ASSOC, SEP_CLAUSES, SEP_EXISTS_THM,
      HCOND_EXTRACT] >>
   EQ_TAC >> rpt DISCH_TAC
   >-(mp_tac UNIQUE_STDIO >> disch_then drule >>
@@ -129,8 +116,7 @@ Proof
   qexists_tac`u0` >> qexists_tac`v0` >> fs[] >>
   qexists_tac`u1` >> fs[PULL_EXISTS] >> qexists_tac`ll` >> fs[] >>
   cases_on`fs1` >> cases_on`fs2` >> fs[IO_fs_numchars_fupd] >>
-  metis_tac[]
-QED
+  metis_tac[]);
 
 (* refinement invariant for filenames *)
 
@@ -143,63 +129,42 @@ val FILENAME_def = Define `
 
 val filename_tac = metis_tac[FILENAME_def,EqualityType_NUM_BOOL,EqualityType_def];
 
-Theorem FILENAME_UNICITY_R[xlet_auto_match]:
- !f fv fv'. FILENAME f fv ==> (FILENAME f fv' <=> fv' = fv)
-Proof
-filename_tac
-QED
+Theorem FILENAME_UNICITY_R[xlet_auto_match]
+`!f fv fv'. FILENAME f fv ==> (FILENAME f fv' <=> fv' = fv)` (filename_tac);
 
-Theorem FILENAME_UNICITY_L[xlet_auto_match]:
- !f f' fv. FILENAME f fv ==> (FILENAME f' fv <=> f' = f)
-Proof
-filename_tac
-QED
+Theorem FILENAME_UNICITY_L[xlet_auto_match]
+`!f f' fv. FILENAME f fv ==> (FILENAME f' fv <=> f' = f)` (filename_tac);
 
-Theorem FILENAME_STRING_UNICITY_R[xlet_auto_match]:
-   !f fv fv'. FILENAME f fv ==> (STRING_TYPE f fv' <=> fv' = fv)
-Proof
-  filename_tac
-QED
+Theorem FILENAME_STRING_UNICITY_R[xlet_auto_match]
+  `!f fv fv'. FILENAME f fv ==> (STRING_TYPE f fv' <=> fv' = fv)`
+  (filename_tac);
 
-Theorem FILENAME_STRING_UNICITY_L[xlet_auto_match]:
-   !f f' fv. FILENAME f fv ==> (STRING_TYPE f' fv <=> f' = f)
-Proof
-filename_tac
-QED
+Theorem FILENAME_STRING_UNICITY_L[xlet_auto_match]
+  `!f f' fv. FILENAME f fv ==> (STRING_TYPE f' fv <=> f' = f)` (filename_tac);
 
-Theorem STRING_FILENAME_UNICITY_R[xlet_auto_match]:
-   !f fv fv'. STRING_TYPE f fv ==>
-    (FILENAME f fv' <=> fv' = fv /\ ¬MEM #"\^@" (explode f) /\ strlen f < 256 * 256)
-Proof
-  filename_tac
-QED
+Theorem STRING_FILENAME_UNICITY_R[xlet_auto_match]
+  `!f fv fv'. STRING_TYPE f fv ==>
+    (FILENAME f fv' <=> fv' = fv /\ ¬MEM #"\^@" (explode f) /\ strlen f < 256 * 256)`
+  (filename_tac);
 
-Theorem STRING_FILENAME_UNICITY_L[xlet_auto_match]:
-   !f f' fv. STRING_TYPE f fv ==>
-    (FILENAME f' fv <=> f' = f /\ ¬MEM #"\^@" (explode f) /\ strlen f < 256 * 256)
-Proof
-  filename_tac
-QED
+Theorem STRING_FILENAME_UNICITY_L[xlet_auto_match]
+  `!f f' fv. STRING_TYPE f fv ==>
+    (FILENAME f' fv <=> f' = f /\ ¬MEM #"\^@" (explode f) /\ strlen f < 256 * 256)`
+  (filename_tac);
 
 (* exception refinement invariant lemmas *)
 
-Theorem BadFileName_UNICITY[xlet_auto_match]:
- !v1 v2. BadFileName_exn v1 ==> (BadFileName_exn v2 <=> v2 = v1)
-Proof
-  fs[BadFileName_exn_def]
-QED
+Theorem BadFileName_UNICITY[xlet_auto_match]
+`!v1 v2. BadFileName_exn v1 ==> (BadFileName_exn v2 <=> v2 = v1)`
+  (fs[BadFileName_exn_def]);
 
-Theorem InvalidFD_UNICITY[xlet_auto_match]:
- !v1 v2. InvalidFD_exn v1 ==> (InvalidFD_exn v2 <=> v2 = v1)
-Proof
-  fs[InvalidFD_exn_def]
-QED
+Theorem InvalidFD_UNICITY[xlet_auto_match]
+`!v1 v2. InvalidFD_exn v1 ==> (InvalidFD_exn v2 <=> v2 = v1)`
+  (fs[InvalidFD_exn_def]);
 
-Theorem EndOfFile_UNICITY[xlet_auto_match]:
- !v1 v2. EndOfFile_exn v1 ==> (EndOfFile_exn v2 <=> v2 = v1)
-Proof
-  fs[EndOfFile_exn_def]
-QED
+Theorem EndOfFile_UNICITY[xlet_auto_match]
+`!v1 v2. EndOfFile_exn v1 ==> (EndOfFile_exn v2 <=> v2 = v1)`
+  (fs[EndOfFile_exn_def]);
 
 Theorem IllegalArgument_UNICITY[xlet_auto_match]
 `!v1 v2. IllegalArgument_exn v1 ==> (IllegalArgument_exn v2 <=> v2 = v1)`
@@ -210,455 +175,339 @@ Theorem IllegalArgument_UNICITY[xlet_auto_match]
 
 val stdo_def = Define`
   stdo fd name fs out =
-    (ALOOKUP fs.infds fd = SOME(UStream(strlit name),WriteMode,strlen out) /\
-     ALOOKUP fs.inode_tbl (UStream(strlit name)) = SOME (explode out))`;
+    (ALOOKUP fs.infds fd = SOME(IOStream(strlit name),WriteMode,strlen out) /\
+     ALOOKUP fs.files (IOStream(strlit name)) = SOME (explode out))`;
 
-Overload stdout = ``stdo 1 "stdout"``
-Overload stderr = ``stdo 2 "stderr"``
+val _ = overload_on("stdout",``stdo 1 "stdout"``);
+val _ = overload_on("stderr",``stdo 2 "stderr"``);
 
-Theorem stdo_UNICITY_R[xlet_auto_match]:
- !fd name fs out out'. stdo fd name fs out ==> (stdo fd name fs out' <=> out = out')
-Proof
-rw[stdo_def] >> EQ_TAC >> rw[explode_11]
-QED
+Theorem stdo_UNICITY_R[xlet_auto_match]
+`!fd name fs out out'. stdo fd name fs out ==> (stdo fd name fs out' <=> out = out')`
+(rw[stdo_def] >> EQ_TAC >> rw[explode_11]);
 
 val up_stdo_def = Define
 `up_stdo fd fs out = fsupdate fs fd 0 (strlen out) (explode out)`
+val _ = overload_on("up_stdout",``up_stdo 1``);
+val _ = overload_on("up_stderr",``up_stdo 2``);
 
-Overload up_stdout = ``up_stdo 1``;
-Overload up_stderr = ``up_stdo 2``;
+Theorem stdo_numchars
+  `stdo fd name (fs with numchars := l) out ⇔ stdo fd name fs out`
+  (rw[stdo_def]);
 
-Theorem stdo_numchars:
-   stdo fd name (fs with numchars := l) out ⇔ stdo fd name fs out
-Proof
-  rw[stdo_def]
-QED
+Theorem up_stdo_numchars[simp]
+  `(up_stdo fd fs x).numchars = fs.numchars`
+  (rw[up_stdo_def,fsupdate_def]
+  \\ CASE_TAC \\ CASE_TAC \\ rw[]);
 
-Theorem up_stdo_numchars[simp]:
-   (up_stdo fd fs x).numchars = fs.numchars
-Proof
-  rw[up_stdo_def,fsupdate_def]
-  \\ CASE_TAC \\ CASE_TAC \\ rw[]
-QED
+Theorem up_stdo_maxFD[simp]
+  `(up_stdo fd fs x).maxFD = fs.maxFD`
+  (rw[up_stdo_def,fsupdate_def]
+  \\ CASE_TAC \\ CASE_TAC \\ rw[]);
 
-Theorem fsupdate_files[simp]:
-  (fsupdate fs fd k pos c).files = fs.files
-Proof
- fs[fsupdate_def] >> NTAC 2 CASE_TAC >>fs[]
-QED
-
-Theorem up_stdo_files[simp]:
-  (up_stdo fd fs x).files = fs.files
-Proof
- fs[up_stdo_def,fsupdate_def] >> NTAC 2 CASE_TAC >>fs[]
-QED
-
-Theorem up_stdo_maxFD[simp]:
-   (up_stdo fd fs x).maxFD = fs.maxFD
-Proof
-  rw[up_stdo_def,fsupdate_def]
-  \\ CASE_TAC \\ CASE_TAC \\ rw[]
-QED
-
-Theorem up_stdo_with_numchars:
-   up_stdo fd (fs with numchars := ns) x =
-   up_stdo fd fs x with numchars := ns
-Proof
-  rw[up_stdo_def,fsupdate_numchars]
-QED
+Theorem up_stdo_with_numchars
+  `up_stdo fd (fs with numchars := ns) x =
+   up_stdo fd fs x with numchars := ns`
+  (rw[up_stdo_def,fsupdate_numchars]);
 
 val add_stdo_def = Define`
   add_stdo fd nm fs out = up_stdo fd fs ((@init. stdo fd nm fs init) ^ out)`;
+val _ = overload_on("add_stdout",``add_stdo 1 "stdout"``);
+val _ = overload_on("add_stderr",``add_stdo 2 "stderr"``);
 
-Overload add_stdout = ``add_stdo 1 "stdout"``
-Overload add_stderr = ``add_stdo 2 "stderr"``
-
-Theorem stdo_add_stdo:
-   stdo fd nm fs init ⇒ stdo fd nm (add_stdo fd nm fs out) (strcat init out)
-Proof
-  rw[add_stdo_def]
+Theorem stdo_add_stdo
+  `stdo fd nm fs init ⇒ stdo fd nm (add_stdo fd nm fs out) (strcat init out)`
+  (rw[add_stdo_def]
   \\ SELECT_ELIM_TAC \\ rw[] >- metis_tac[]
   \\ imp_res_tac stdo_UNICITY_R \\ rveq
-  \\ fs[up_stdo_def,stdo_def,fsupdate_def,AFUPDKEY_ALOOKUP]
-QED
+  \\ fs[up_stdo_def,stdo_def,fsupdate_def,ALIST_FUPDKEY_ALOOKUP]);
 
-Theorem up_stdo_unchanged:
-  !fs out. stdo fd nm fs out ==> up_stdo fd fs out = fs
-Proof
-fs[up_stdo_def,stdo_def,fsupdate_unchanged,get_file_content_def,PULL_EXISTS]
-QED
+Theorem up_stdo_unchanged
+ `!fs out. stdo fd nm fs out ==> up_stdo fd fs out = fs`
+(fs[up_stdo_def,stdo_def,fsupdate_unchanged,get_file_content_def,PULL_EXISTS]);
 
-Theorem stdo_up_stdo:
-  !fs out out'. stdo fd nm fs out ==> stdo fd nm (up_stdo fd fs out') out'
-Proof
- rw[up_stdo_def,stdo_def,fsupdate_def,AFUPDKEY_ALOOKUP,PULL_EXISTS]
- \\ rw[]
-QED
+Theorem stdo_up_stdo
+ `!fs out out'. stdo fd nm fs out ==> stdo fd nm (up_stdo fd fs out') out'`
+ (rw[up_stdo_def,stdo_def,fsupdate_def,ALIST_FUPDKEY_ALOOKUP,PULL_EXISTS]
+ \\ rw[]);
 
-Theorem add_stdo_nil:
-   stdo fd nm fs out ⇒ add_stdo fd nm fs (strlit "") = fs
-Proof
-  rw[add_stdo_def]
+Theorem add_stdo_nil
+  `stdo fd nm fs out ⇒ add_stdo fd nm fs (strlit "") = fs`
+  (rw[add_stdo_def]
   \\ SELECT_ELIM_TAC
-  \\ metis_tac[up_stdo_unchanged]
-QED
+  \\ metis_tac[up_stdo_unchanged]);
 
-Theorem add_stdo_o:
-   stdo fd nm fs out ⇒
-   add_stdo fd nm (add_stdo fd nm fs x1) x2 = add_stdo fd nm fs (x1 ^ x2)
-Proof
-  rw[add_stdo_def]
+Theorem add_stdo_o
+  `stdo fd nm fs out ⇒
+   add_stdo fd nm (add_stdo fd nm fs x1) x2 = add_stdo fd nm fs (x1 ^ x2)`
+  (rw[add_stdo_def]
   \\ SELECT_ELIM_TAC \\ rw[] >- metis_tac[]
   \\ SELECT_ELIM_TAC \\ rw[] >- metis_tac[stdo_up_stdo]
   \\ imp_res_tac stdo_UNICITY_R \\ rveq
   \\ rename1`stdo _ _ (up_stdo _ _ _) l`
   \\ `l = out ^ x1` by metis_tac[stdo_UNICITY_R,stdo_up_stdo]
-  \\ rveq \\ fs[up_stdo_def]
-QED
+  \\ rveq \\ fs[up_stdo_def]);
 
-Theorem add_stdo_numchars[simp]:
-   (add_stdo fd nm fs x).numchars = fs.numchars
-Proof
-  rw[add_stdo_def]
-QED
+Theorem add_stdo_numchars[simp]
+  `(add_stdo fd nm fs x).numchars = fs.numchars`
+  (rw[add_stdo_def]);
 
-Theorem add_stdo_maxFD[simp]:
-   (add_stdo fd nm fs x).maxFD = fs.maxFD
-Proof
-  rw[add_stdo_def]
-QED
+Theorem add_stdo_maxFD[simp]
+  `(add_stdo fd nm fs x).maxFD = fs.maxFD`
+  (rw[add_stdo_def]);
 
-Theorem add_stdo_with_numchars:
-   add_stdo fd nm (fs with numchars := ns) x =
-   add_stdo fd nm fs x with numchars := ns
-Proof
-  rw[add_stdo_def,stdo_numchars,up_stdo_with_numchars]
-QED
+Theorem add_stdo_with_numchars
+  `add_stdo fd nm (fs with numchars := ns) x =
+   add_stdo fd nm fs x with numchars := ns`
+  (rw[add_stdo_def,stdo_numchars,up_stdo_with_numchars]);
 
-Theorem up_stdo_MAP_FST_infds[simp]:
-   MAP FST (up_stdo fd fs out).infds = MAP FST fs.infds
-Proof
-  rw[up_stdo_def]
-QED
+Theorem up_stdo_MAP_FST_infds[simp]
+  `MAP FST (up_stdo fd fs out).infds = MAP FST fs.infds`
+  (rw[up_stdo_def]);
 
-Theorem add_stdo_MAP_FST_infds[simp]:
-   MAP FST (add_stdo fd nm fs out).infds = MAP FST fs.infds
-Proof
-  rw[add_stdo_def]
-QED
+Theorem add_stdo_MAP_FST_infds[simp]
+  `MAP FST (add_stdo fd nm fs out).infds = MAP FST fs.infds`
+  (rw[add_stdo_def]);
 
-Theorem up_stdo_MAP_FST_files[simp]:
-   MAP FST (up_stdo fd fs out).files = MAP FST fs.files
-Proof
-  rw[up_stdo_def]
-QED
+Theorem up_stdo_MAP_FST_files[simp]
+  `MAP FST (up_stdo fd fs out).files = MAP FST fs.files`
+  (rw[up_stdo_def]);
 
-Theorem up_stdo_MAP_FST_inode_tbl[simp]:
-   MAP FST (up_stdo fd fs out).inode_tbl = MAP FST fs.inode_tbl
-Proof
-  rw[up_stdo_def]
-QED
+Theorem add_stdo_MAP_FST_files[simp]
+  `MAP FST (add_stdo fd nm fs out).files = MAP FST fs.files`
+  (rw[add_stdo_def]);
 
-Theorem add_stdo_MAP_FST_inode_tbl[simp]:
-   MAP FST (add_stdo fd nm fs out).inode_tbl = MAP FST fs.inode_tbl
-Proof
-  rw[add_stdo_def]
-QED
+Theorem inFS_fname_add_stdo[simp]
+  `inFS_fname (add_stdo fd nm fs out) = inFS_fname fs`
+  (rw[inFS_fname_def,FUN_EQ_THM]);
 
-Theorem inFS_fname_add_stdo[simp]:
-   inFS_fname (add_stdo fd nm fs out) = inFS_fname fs
-Proof
-  rw[inFS_fname_def,FUN_EQ_THM] >> EVAL_TAC >> EVERY_CASE_TAC >> rw[]
-QED
+Theorem STD_streams_stdout
+  `STD_streams fs ⇒ ∃out. stdout fs out`
+  (rw[STD_streams_def,stdo_def] \\ rw[] \\ metis_tac[explode_implode,strlen_implode]);
 
-Theorem STD_streams_stdout:
-   STD_streams fs ⇒ ∃out. stdout fs out
-Proof
-  rw[STD_streams_def,stdo_def] \\ rw[] \\ metis_tac[explode_implode,strlen_implode]
-QED
+Theorem STD_streams_stderr
+  `STD_streams fs ⇒ ∃out. stderr fs out`
+  (rw[STD_streams_def,stdo_def] \\ rw[] \\ metis_tac[explode_implode,strlen_implode]);
 
-Theorem STD_streams_stderr:
-   STD_streams fs ⇒ ∃out. stderr fs out
-Proof
-  rw[STD_streams_def,stdo_def] \\ rw[] \\ metis_tac[explode_implode,strlen_implode]
-QED
-
-Theorem STD_streams_add_stdout:
-   STD_streams fs ⇒ STD_streams (add_stdout fs out)
-Proof
-  rw[]
+Theorem STD_streams_add_stdout
+  `STD_streams fs ⇒ STD_streams (add_stdout fs out)`
+  (rw[]
   \\ imp_res_tac STD_streams_stdout
   \\ rw[add_stdo_def]
   \\ SELECT_ELIM_TAC
   \\ rw[] >- metis_tac[]
   \\ rw[up_stdo_def]
-  \\ match_mp_tac STD_streams_fsupdate \\ rw[]
-QED
+  \\ match_mp_tac STD_streams_fsupdate \\ rw[]);
 
-Theorem STD_streams_add_stderr:
-   STD_streams fs ⇒ STD_streams (add_stderr fs out)
-Proof
-  rw[]
+Theorem STD_streams_add_stderr
+  `STD_streams fs ⇒ STD_streams (add_stderr fs out)`
+  (rw[]
   \\ imp_res_tac STD_streams_stderr
   \\ rw[add_stdo_def]
   \\ SELECT_ELIM_TAC
   \\ rw[] >- metis_tac[]
   \\ rw[up_stdo_def]
-  \\ match_mp_tac STD_streams_fsupdate \\ rw[]
-QED
+  \\ match_mp_tac STD_streams_fsupdate \\ rw[]);
 
-Theorem validFD_up_stdo[simp]:
-   validFD fd (up_stdo fd' fs out) ⇔ validFD fd fs
-Proof
-  rw[up_stdo_def]
-QED
+Theorem validFD_up_stdo[simp]
+  `validFD fd (up_stdo fd' fs out) ⇔ validFD fd fs`
+  (rw[up_stdo_def]);
 
-Theorem validFD_add_stdo[simp]:
-   validFD fd (add_stdo fd' nm fs out) ⇔ validFD fd fs
-Proof
-  rw[add_stdo_def]
-QED
+Theorem validFD_add_stdo[simp]
+  `validFD fd (add_stdo fd' nm fs out) ⇔ validFD fd fs`
+  (rw[add_stdo_def]);
 
-Theorem validFileFD_up_stdo[simp]:
-   validFileFD fd (up_stdo fd' fs out).infds ⇔ validFileFD fd fs.infds
-Proof
-  rw[up_stdo_def]
-QED
+Theorem validFileFD_up_stdo[simp]
+  `validFileFD fd (up_stdo fd' fs out).infds ⇔ validFileFD fd fs.infds`
+  (rw[up_stdo_def]);
 
-Theorem validFileFD_add_stdo[simp]:
-   validFileFD fd (add_stdo fd' nm fs out).infds ⇔ validFileFD fd fs.infds
-Proof
-  rw[add_stdo_def]
-QED
+Theorem validFileFD_add_stdo[simp]
+  `validFileFD fd (add_stdo fd' nm fs out).infds ⇔ validFileFD fd fs.infds`
+  (rw[add_stdo_def]);
 
-Theorem up_stdo_ADELKEY:
-   fd ≠ fd' ⇒
-   up_stdo fd (fs with infds updated_by ADELKEY fd') out =
-   up_stdo fd fs out with infds updated_by ADELKEY fd'
-Proof
-  rw[up_stdo_def,fsupdate_ADELKEY]
-QED
+Theorem up_stdo_A_DELKEY
+  `fd ≠ fd' ⇒
+   up_stdo fd (fs with infds updated_by A_DELKEY fd') out =
+   up_stdo fd fs out with infds updated_by A_DELKEY fd'`
+  (rw[up_stdo_def,fsupdate_A_DELKEY]);
 
-Theorem stdo_ADELKEY:
-   fd ≠ fd' ⇒
-   stdo fd nm (fs with infds updated_by ADELKEY fd') = stdo fd nm fs
-Proof
-  rw[stdo_def,FUN_EQ_THM,ALOOKUP_ADELKEY]
-QED
+Theorem stdo_A_DELKEY
+  `fd ≠ fd' ⇒
+   stdo fd nm (fs with infds updated_by A_DELKEY fd') = stdo fd nm fs`
+  (rw[stdo_def,FUN_EQ_THM,ALOOKUP_ADELKEY]);
 
-Theorem add_stdo_ADELKEY:
-   fd ≠ fd' ⇒
-   add_stdo fd nm (fs with infds updated_by ADELKEY fd') out =
-   add_stdo fd nm fs out with infds updated_by ADELKEY fd'
-Proof
-  rw[add_stdo_def,up_stdo_ADELKEY,stdo_ADELKEY]
-QED
+Theorem add_stdo_A_DELKEY
+  `fd ≠ fd' ⇒
+   add_stdo fd nm (fs with infds updated_by A_DELKEY fd') out =
+   add_stdo fd nm fs out with infds updated_by A_DELKEY fd'`
+  (rw[add_stdo_def,up_stdo_A_DELKEY,stdo_A_DELKEY]);
 
-Theorem get_file_content_add_stdout:
-   STD_streams fs ∧ fd ≠ 1 ⇒
-   get_file_content (add_stdout fs out) fd = get_file_content fs fd
-Proof
-  rw[get_file_content_def,add_stdo_def,up_stdo_def,fsupdate_def]
-  \\ CASE_TAC \\ CASE_TAC \\ simp[AFUPDKEY_ALOOKUP]
+Theorem get_file_content_add_stdout
+  `STD_streams fs ∧ fd ≠ 1 ⇒
+   get_file_content (add_stdout fs out) fd = get_file_content fs fd`
+  (rw[get_file_content_def,add_stdo_def,up_stdo_def,fsupdate_def]
+  \\ CASE_TAC \\ CASE_TAC \\ simp[ALIST_FUPDKEY_ALOOKUP]
   \\ TOP_CASE_TAC \\ fs[]
   \\ pairarg_tac \\ fs[]
   \\ CASE_TAC
   >- metis_tac[STD_streams_def,SOME_11,PAIR,FST,SND]
-  \\ CASE_TAC
-QED
+  \\ CASE_TAC);
 
-Theorem get_mode_add_stdo[simp]:
-   get_mode (add_stdo fd nm fs x) fd' = get_mode fs fd'
-Proof
-  rw[get_mode_def,add_stdo_def, up_stdo_def, fsupdate_def]
+Theorem get_mode_add_stdo[simp]
+  `get_mode (add_stdo fd nm fs x) fd' = get_mode fs fd'`
+  (rw[get_mode_def,add_stdo_def, up_stdo_def, fsupdate_def]
   \\ TOP_CASE_TAC \\ rw[]
   \\ TOP_CASE_TAC \\ rw[]
-  \\ simp[AFUPDKEY_ALOOKUP]
-  \\ TOP_CASE_TAC \\ rw[]
-QED
+  \\ simp[ALIST_FUPDKEY_ALOOKUP]
+  \\ TOP_CASE_TAC \\ rw[]);
 
-Theorem get_mode_bumpFD[simp]:
-   get_mode (bumpFD fd fs n) fd' = get_mode fs fd'
-Proof
-  rw[get_mode_def,bumpFD_def,AFUPDKEY_ALOOKUP]
-  \\ TOP_CASE_TAC \\ rw[]
-QED
+Theorem get_mode_bumpFD[simp]
+  `get_mode (bumpFD fd fs n) fd' = get_mode fs fd'`
+  (rw[get_mode_def,bumpFD_def,ALIST_FUPDKEY_ALOOKUP]
+  \\ TOP_CASE_TAC \\ rw[]);
 
-Theorem linesFD_add_stdout:
-   STD_streams fs ∧ fd ≠ 1 ⇒
-   linesFD (add_stdout fs out) fd = linesFD fs fd
-Proof
-  rw[linesFD_def,get_file_content_add_stdout]
-QED
+Theorem linesFD_add_stdout
+  `STD_streams fs ∧ fd ≠ 1 ⇒
+   linesFD (add_stdout fs out) fd = linesFD fs fd`
+  (rw[linesFD_def,get_file_content_add_stdout]);
 
-Theorem get_file_content_add_stderr:
-   STD_streams fs ∧ fd ≠ 2 ⇒
-   get_file_content (add_stderr fs err) fd = get_file_content fs fd
-Proof
-  rw[get_file_content_def,add_stdo_def,up_stdo_def,fsupdate_def]
-  \\ CASE_TAC \\ CASE_TAC \\ simp[AFUPDKEY_ALOOKUP]
+Theorem get_file_content_add_stderr
+  `STD_streams fs ∧ fd ≠ 2 ⇒
+   get_file_content (add_stderr fs err) fd = get_file_content fs fd`
+  (rw[get_file_content_def,add_stdo_def,up_stdo_def,fsupdate_def]
+  \\ CASE_TAC \\ CASE_TAC \\ simp[ALIST_FUPDKEY_ALOOKUP]
   \\ TOP_CASE_TAC \\ fs[]
   \\ pairarg_tac \\ fs[]
   \\ CASE_TAC
   >- metis_tac[STD_streams_def,SOME_11,PAIR,FST,SND]
-  \\ CASE_TAC
-QED
+  \\ CASE_TAC);
 
-Theorem linesFD_add_stderr:
-   STD_streams fs ∧ fd ≠ 2 ⇒
-   linesFD (add_stderr fs err) fd = linesFD fs fd
-Proof
-  rw[linesFD_def,get_file_content_add_stderr]
-QED
+Theorem linesFD_add_stderr
+  `STD_streams fs ∧ fd ≠ 2 ⇒
+   linesFD (add_stderr fs err) fd = linesFD fs fd`
+  (rw[linesFD_def,get_file_content_add_stderr]);
 
-Theorem up_stdo_forwardFD:
-   fd ≠ fd' ⇒ up_stdo fd' (forwardFD fs fd n) out = forwardFD (up_stdo fd' fs out) fd n
-Proof
-  rw[forwardFD_def,up_stdo_def,fsupdate_def,AFUPDKEY_ALOOKUP]
+Theorem up_stdo_forwardFD
+  `fd ≠ fd' ⇒ up_stdo fd' (forwardFD fs fd n) out = forwardFD (up_stdo fd' fs out) fd n`
+  (rw[forwardFD_def,up_stdo_def,fsupdate_def,ALIST_FUPDKEY_ALOOKUP]
   \\ CASE_TAC \\ CASE_TAC \\ rw[]
   \\ rpt(AP_TERM_TAC ORELSE AP_THM_TAC)
-  \\ match_mp_tac AFUPDKEY_comm \\ rw[]
-QED
+  \\ match_mp_tac ALIST_FUPDKEY_comm \\ rw[]);
 
-Theorem up_stdout_fastForwardFD:
-   STD_streams fs ⇒
-   up_stdout (fastForwardFD fs fd) out = fastForwardFD (up_stdout fs out) fd
-Proof
-  rw[fastForwardFD_def,up_stdo_def]
+Theorem up_stdout_fastForwardFD
+  `STD_streams fs ⇒
+   up_stdout (fastForwardFD fs fd) out = fastForwardFD (up_stdout fs out) fd`
+  (rw[fastForwardFD_def,up_stdo_def]
   \\ Cases_on`ALOOKUP fs.infds fd` >- (
     fs[libTheory.the_def,fsupdate_def]
     \\ CASE_TAC \\ fs[libTheory.the_def]
-    \\ CASE_TAC \\ fs[libTheory.the_def,AFUPDKEY_ALOOKUP] )
+    \\ CASE_TAC \\ fs[libTheory.the_def,ALIST_FUPDKEY_ALOOKUP] )
   \\ fs[] \\ pairarg_tac \\ fs[]
-  \\ Cases_on`ALOOKUP fs.inode_tbl ino` >- (
+  \\ Cases_on`ALOOKUP fs.files fnm` >- (
     fs[libTheory.the_def,fsupdate_def]
     \\ CASE_TAC \\ fs[libTheory.the_def]
-    \\ CASE_TAC \\ fs[libTheory.the_def,AFUPDKEY_ALOOKUP]
+    \\ CASE_TAC \\ fs[libTheory.the_def,ALIST_FUPDKEY_ALOOKUP]
     \\ rw[libTheory.the_def] )
   \\ fs[libTheory.the_def]
-  \\ fs[fsupdate_def,libTheory.the_def,AFUPDKEY_ALOOKUP]
-  \\ CASE_TAC \\ fs[libTheory.the_def,AFUPDKEY_ALOOKUP]
-  >- ( rw[AFUPDKEY_o,o_DEF,PAIR_MAP] )
+  \\ fs[fsupdate_def,libTheory.the_def,ALIST_FUPDKEY_ALOOKUP]
+  \\ CASE_TAC \\ fs[libTheory.the_def,ALIST_FUPDKEY_ALOOKUP]
+  >- ( rw[ALIST_FUPDKEY_o,o_DEF,PAIR_MAP] )
   \\ CASE_TAC \\ fs[libTheory.the_def]
-  \\ CASE_TAC \\ fs[libTheory.the_def,AFUPDKEY_ALOOKUP]
-  \\ rw[libTheory.the_def,AFUPDKEY_comm]
-  \\ metis_tac[STD_streams_def,SOME_11,PAIR,FST,SND]
-QED
+  \\ CASE_TAC \\ fs[libTheory.the_def,ALIST_FUPDKEY_ALOOKUP]
+  \\ rw[libTheory.the_def,ALIST_FUPDKEY_comm]
+  \\ metis_tac[STD_streams_def,SOME_11,PAIR,FST,SND]);
 
-Theorem up_stderr_fastForwardFD:
-   STD_streams fs ⇒
-   up_stderr (fastForwardFD fs fd) out = fastForwardFD (up_stderr fs out) fd
-Proof
-  rw[fastForwardFD_def,up_stdo_def]
+Theorem up_stderr_fastForwardFD
+  `STD_streams fs ⇒
+   up_stderr (fastForwardFD fs fd) out = fastForwardFD (up_stderr fs out) fd`
+  (rw[fastForwardFD_def,up_stdo_def]
   \\ Cases_on`ALOOKUP fs.infds fd` >- (
     fs[libTheory.the_def,fsupdate_def]
     \\ CASE_TAC \\ fs[libTheory.the_def]
-    \\ CASE_TAC \\ fs[libTheory.the_def,AFUPDKEY_ALOOKUP] )
+    \\ CASE_TAC \\ fs[libTheory.the_def,ALIST_FUPDKEY_ALOOKUP] )
   \\ fs[] \\ pairarg_tac \\ fs[]
-  \\ Cases_on`ALOOKUP fs.inode_tbl ino` >- (
+  \\ Cases_on`ALOOKUP fs.files fnm` >- (
     fs[libTheory.the_def,fsupdate_def]
     \\ CASE_TAC \\ fs[libTheory.the_def]
-    \\ CASE_TAC \\ fs[libTheory.the_def,AFUPDKEY_ALOOKUP]
+    \\ CASE_TAC \\ fs[libTheory.the_def,ALIST_FUPDKEY_ALOOKUP]
     \\ rw[libTheory.the_def] )
   \\ fs[libTheory.the_def]
-  \\ fs[fsupdate_def,libTheory.the_def,AFUPDKEY_ALOOKUP]
-  \\ CASE_TAC \\ fs[libTheory.the_def,AFUPDKEY_ALOOKUP]
-  >- ( rw[AFUPDKEY_o,o_DEF,PAIR_MAP] )
+  \\ fs[fsupdate_def,libTheory.the_def,ALIST_FUPDKEY_ALOOKUP]
+  \\ CASE_TAC \\ fs[libTheory.the_def,ALIST_FUPDKEY_ALOOKUP]
+  >- ( rw[ALIST_FUPDKEY_o,o_DEF,PAIR_MAP] )
   \\ CASE_TAC \\ fs[libTheory.the_def]
-  \\ CASE_TAC \\ fs[libTheory.the_def,AFUPDKEY_ALOOKUP]
-  \\ rw[libTheory.the_def,AFUPDKEY_comm]
-  \\ metis_tac[STD_streams_def,SOME_11,PAIR,FST,SND]
-QED
+  \\ CASE_TAC \\ fs[libTheory.the_def,ALIST_FUPDKEY_ALOOKUP]
+  \\ rw[libTheory.the_def,ALIST_FUPDKEY_comm]
+  \\ metis_tac[STD_streams_def,SOME_11,PAIR,FST,SND]);
 
-Theorem stdo_forwardFD:
-   fd ≠ fd' ⇒ (stdo fd' nm (forwardFD fs fd n) out ⇔ stdo fd' nm fs out)
-Proof
-  rw[stdo_def,forwardFD_def,AFUPDKEY_ALOOKUP]
-  \\ CASE_TAC
-QED
+Theorem stdo_forwardFD
+  `fd ≠ fd' ⇒ (stdo fd' nm (forwardFD fs fd n) out ⇔ stdo fd' nm fs out)`
+  (rw[stdo_def,forwardFD_def,ALIST_FUPDKEY_ALOOKUP]
+  \\ CASE_TAC);
 
-Theorem stdo_fastForwardFD:
-   fd ≠ fd' ⇒ (stdo fd' nm (fastForwardFD fs fd) out ⇔ stdo fd' nm fs out)
-Proof
-  rw[stdo_def,fastForwardFD_def,AFUPDKEY_ALOOKUP]
+Theorem stdo_fastForwardFD
+  `fd ≠ fd' ⇒ (stdo fd' nm (fastForwardFD fs fd) out ⇔ stdo fd' nm fs out)`
+  (rw[stdo_def,fastForwardFD_def,ALIST_FUPDKEY_ALOOKUP]
   \\ Cases_on`ALOOKUP fs.infds fd` \\ fs[libTheory.the_def]
   \\ pairarg_tac \\ fs[]
-  \\ Cases_on`ALOOKUP fs.inode_tbl ino` \\ fs[libTheory.the_def]
-  \\ fs[AFUPDKEY_ALOOKUP] \\ rw[]
-  \\ CASE_TAC
-QED
+  \\ Cases_on`ALOOKUP fs.files fnm` \\ fs[libTheory.the_def]
+  \\ fs[ALIST_FUPDKEY_ALOOKUP] \\ rw[]
+  \\ CASE_TAC);
 
-Theorem add_stdo_forwardFD:
-   fd ≠ fd' ⇒ add_stdo fd' nm (forwardFD fs fd n) out = forwardFD (add_stdo fd' nm fs out) fd n
-Proof
-  rw[add_stdo_def,stdo_forwardFD,up_stdo_forwardFD]
-QED
+Theorem add_stdo_forwardFD
+  `fd ≠ fd' ⇒ add_stdo fd' nm (forwardFD fs fd n) out = forwardFD (add_stdo fd' nm fs out) fd n`
+  (rw[add_stdo_def,stdo_forwardFD,up_stdo_forwardFD]);
 
-Theorem add_stdout_lineForwardFD:
-   STD_streams fs ∧ fd ≠ 1 ⇒
-   add_stdout (lineForwardFD fs fd) out = lineForwardFD (add_stdout fs out) fd
-Proof
-  rw[lineForwardFD_def,get_file_content_add_stdout]
+Theorem add_stdout_lineForwardFD
+  `STD_streams fs ∧ fd ≠ 1 ⇒
+   add_stdout (lineForwardFD fs fd) out = lineForwardFD (add_stdout fs out) fd`
+  (rw[lineForwardFD_def,get_file_content_add_stdout]
   \\ CASE_TAC \\ CASE_TAC
-  \\ rw[] \\ pairarg_tac \\ fs[add_stdo_forwardFD]
-QED
+  \\ rw[] \\ pairarg_tac \\ fs[add_stdo_forwardFD]);
 
-Theorem add_stdout_fastForwardFD:
-   STD_streams fs ∧ fd ≠ 1 ⇒
-   add_stdout (fastForwardFD fs fd) out = fastForwardFD (add_stdout fs out) fd
-Proof
-  rw[add_stdo_def,up_stdout_fastForwardFD,stdo_fastForwardFD]
-QED
+Theorem add_stdout_fastForwardFD
+  `STD_streams fs ∧ fd ≠ 1 ⇒
+   add_stdout (fastForwardFD fs fd) out = fastForwardFD (add_stdout fs out) fd`
+  (rw[add_stdo_def,up_stdout_fastForwardFD,stdo_fastForwardFD]);
 
-Theorem add_stderr_lineForwardFD:
-   STD_streams fs ∧ fd ≠ 2 ⇒
-   add_stderr (lineForwardFD fs fd) out = lineForwardFD (add_stderr fs out) fd
-Proof
-  rw[lineForwardFD_def,get_file_content_add_stderr]
+Theorem add_stderr_lineForwardFD
+  `STD_streams fs ∧ fd ≠ 2 ⇒
+   add_stderr (lineForwardFD fs fd) out = lineForwardFD (add_stderr fs out) fd`
+  (rw[lineForwardFD_def,get_file_content_add_stderr]
   \\ CASE_TAC \\ CASE_TAC
-  \\ rw[] \\ pairarg_tac \\ fs[add_stdo_forwardFD]
-QED
+  \\ rw[] \\ pairarg_tac \\ fs[add_stdo_forwardFD]);
 
-Theorem add_stderr_fastForwardFD:
-   STD_streams fs ∧ fd ≠ 2 ⇒
-   add_stderr (fastForwardFD fs fd) out = fastForwardFD (add_stderr fs out) fd
-Proof
-  rw[add_stdo_def,up_stderr_fastForwardFD,stdo_fastForwardFD]
-QED
+Theorem add_stderr_fastForwardFD
+  `STD_streams fs ∧ fd ≠ 2 ⇒
+   add_stderr (fastForwardFD fs fd) out = fastForwardFD (add_stderr fs out) fd`
+  (rw[add_stdo_def,up_stderr_fastForwardFD,stdo_fastForwardFD]);
 
-Theorem FILTER_File_add_stdo:
-   stdo fd nm fs init ⇒
-   FILTER (isFile o FST) (add_stdo fd nm fs out).inode_tbl = FILTER (isFile o FST) fs.inode_tbl
-Proof
-  rw[add_stdo_def,up_stdo_def,fsupdate_def]
+Theorem FILTER_File_add_stdo
+  `stdo fd nm fs init ⇒
+   FILTER (isFile o FST) (add_stdo fd nm fs out).files = FILTER (isFile o FST) fs.files`
+  (rw[add_stdo_def,up_stdo_def,fsupdate_def]
   \\ CASE_TAC \\ CASE_TAC \\ fs[]
   \\ match_mp_tac FILTER_EL_EQ \\ simp[]
   \\ qmatch_assum_rename_tac`_ = SOME (k,_)`
   \\ qx_gen_tac`n`
   \\ simp[GSYM AND_IMP_INTRO] \\ strip_tac
-  \\ reverse(Cases_on`FST (EL n fs.inode_tbl) = k`)
-  >- simp[EL_AFUPDKEY_unchanged]
-  \\ simp[FST_EL_AFUPDKEY,GSYM AND_IMP_INTRO]
-  \\ fs[stdo_def]
-QED
+  \\ reverse(Cases_on`FST (EL n fs.files) = k`)
+  >- simp[EL_ALIST_FUPDKEY_unchanged]
+  \\ simp[FST_EL_ALIST_FUPDKEY,GSYM AND_IMP_INTRO]
+  \\ fs[stdo_def]);
 
-Theorem FILTER_File_add_stdout:
-   STD_streams fs ⇒
-   FILTER (isFile o FST) (add_stdout fs out).inode_tbl = FILTER (isFile o FST) fs.inode_tbl
-Proof
-  metis_tac[STD_streams_stdout,FILTER_File_add_stdo]
-QED
+Theorem FILTER_File_add_stdout
+  `STD_streams fs ⇒
+   FILTER (isFile o FST) (add_stdout fs out).files = FILTER (isFile o FST) fs.files`
+  (metis_tac[STD_streams_stdout,FILTER_File_add_stdo]);
 
-Theorem FILTER_File_add_stderr:
-   STD_streams fs ⇒
-   FILTER (isFile o FST) (add_stderr fs out).inode_tbl = FILTER (isFile o FST) fs.inode_tbl
-Proof
-  metis_tac[STD_streams_stderr,FILTER_File_add_stdo]
-QED
+Theorem FILTER_File_add_stderr
+  `STD_streams fs ⇒
+   FILTER (isFile o FST) (add_stderr fs out).files = FILTER (isFile o FST) fs.files`
+  (metis_tac[STD_streams_stderr,FILTER_File_add_stdo]);
 
 val stdin_def = Define
-`stdin fs inp pos = (ALOOKUP fs.infds 0 = SOME(UStream(strlit"stdin"),ReadMode,pos) /\
-                     ALOOKUP fs.inode_tbl (UStream(strlit"stdin"))= SOME inp)`
+`stdin fs inp pos = (ALOOKUP fs.infds 0 = SOME(IOStream(strlit"stdin"),ReadMode,pos) /\
+                     ALOOKUP fs.files (IOStream(strlit"stdin"))= SOME inp)`
 
 val up_stdin_def = Define
 `up_stdin inp pos fs = fsupdate fs 0 0 pos inp`
@@ -666,62 +515,50 @@ val up_stdin_def = Define
 val get_stdin_def = Define`
   get_stdin fs = let (inp,pos) = @(inp,pos). stdin fs inp pos in DROP pos inp`;
 
-Theorem stdin_11:
-   stdin fs i1 p1 ∧ stdin fs i2 p2 ⇒ i1 = i2 ∧ p1 = p2
-Proof
-  rw[stdin_def] \\ fs[]
-QED
+Theorem stdin_11
+  `stdin fs i1 p1 ∧ stdin fs i2 p2 ⇒ i1 = i2 ∧ p1 = p2`
+  (rw[stdin_def] \\ fs[]);
 
-Theorem stdin_get_file_content:
-   stdin fs inp pos ⇒ get_file_content fs 0 = SOME (inp,pos)
-Proof
-  rw[stdin_def,fsFFITheory.get_file_content_def]
-QED
+Theorem stdin_get_file_content
+  `stdin fs inp pos ⇒ get_file_content fs 0 = SOME (inp,pos)`
+  (rw[stdin_def,fsFFITheory.get_file_content_def]);
 
-Theorem stdin_forwardFD:
-   stdin fs inp pos ⇒
-   stdin (forwardFD fs fd n) inp (if fd = 0 then pos+n else pos)
-Proof
-  rw[stdin_def,forwardFD_def]
-  \\ simp[AFUPDKEY_ALOOKUP]
-QED
+Theorem stdin_forwardFD
+  `stdin fs inp pos ⇒
+   stdin (forwardFD fs fd n) inp (if fd = 0 then pos+n else pos)`
+  (rw[stdin_def,forwardFD_def]
+  \\ simp[ALIST_FUPDKEY_ALOOKUP]);
 
-Theorem stdin_get_stdin:
-   stdin fs inp pos ⇒ get_stdin fs = DROP pos inp
-Proof
-  rw[get_stdin_def]
+Theorem stdin_get_stdin
+  `stdin fs inp pos ⇒ get_stdin fs = DROP pos inp`
+  (rw[get_stdin_def]
   \\ SELECT_ELIM_TAC
   \\ rw[EXISTS_PROD,FORALL_PROD]
   >- metis_tac[]
   \\ pairarg_tac \\ fs[]
-  \\ imp_res_tac stdin_11 \\ fs[]
-QED
+  \\ imp_res_tac stdin_11 \\ fs[]);
 
-Theorem get_stdin_forwardFD:
-   stdin fs inp pos ⇒
+Theorem get_stdin_forwardFD
+  `stdin fs inp pos ⇒
    get_stdin (forwardFD fs fd n) =
    if fd = 0 then
      DROP n (get_stdin fs)
-   else get_stdin fs
-Proof
-  strip_tac
+   else get_stdin fs`
+  (strip_tac
   \\ imp_res_tac stdin_get_stdin
   \\ imp_res_tac stdin_forwardFD
   \\ first_x_assum(qspecl_then[`n`,`fd`]mp_tac)
   \\ strip_tac
   \\ simp[DROP_DROP_T]
   \\ imp_res_tac stdin_get_stdin
-  \\ rw[]
-QED
+  \\ rw[]);
 
-Theorem linesFD_splitlines_get_stdin:
-   stdin fs inp pos ⇒
-    MAP (λl. l ++ "\n") (splitlines (get_stdin fs)) = linesFD fs 0
-Proof
-  rw[linesFD_def]
+Theorem linesFD_splitlines_get_stdin
+  `stdin fs inp pos ⇒
+   MAP (λl. l ++ "\n") (splitlines (get_stdin fs)) = linesFD fs 0`
+  (rw[linesFD_def]
   \\ imp_res_tac stdin_get_stdin
-  \\ fs[stdin_def,get_file_content_def]
-QED
+  \\ fs[stdin_def,get_file_content_def]);
 
 (* file descriptors are encoded on 8 bytes *)
 val FD_def = Define `
@@ -795,28 +632,22 @@ val OUTSTREAM_def = Define `
     OUTSTREAM_TYPE (Outstream (strlit(MAP (CHR ∘ w2n) (n2w8 fd)))) fdv ∧
     fd < 256**8`
 
-Theorem INSTREAM_stdin:
-   INSTREAM 0 stdin_v
-Proof
-  fs[INSTREAM_def,MarshallingTheory.n2w8_def,stdin_v_thm,GSYM stdIn_def]
-QED
+Theorem INSTREAM_stdin
+  `INSTREAM 0 stdin_v`
+  (fs[INSTREAM_def,MarshallingTheory.n2w8_def,stdin_v_thm,GSYM stdIn_def]);
 
-Theorem OUTSTREAM_stdout:
-   OUTSTREAM 1 stdout_v
-Proof
-  fs[OUTSTREAM_def,MarshallingTheory.n2w8_def,stdout_v_thm,GSYM stdOut_def]
-QED
+Theorem OUTSTREAM_stdout
+  `OUTSTREAM 1 stdout_v`
+  (fs[OUTSTREAM_def,MarshallingTheory.n2w8_def,stdout_v_thm,GSYM stdOut_def]);
 
-Theorem OUTSTREAM_stderr:
-   OUTSTREAM 2 stderr_v
-Proof
-  fs[OUTSTREAM_def,MarshallingTheory.n2w8_def,stderr_v_thm,GSYM stdErr_def]
-QED
+Theorem OUTSTREAM_stderr
+  `OUTSTREAM 2 stderr_v`
+  (fs[OUTSTREAM_def,MarshallingTheory.n2w8_def,stderr_v_thm,GSYM stdErr_def]);
 
 (* -- *)
 
-Theorem openIn_spec:
-   ∀s sv fs.
+Theorem openIn_spec
+  `∀s sv fs.
      FILENAME s sv ∧
      hasFreeFD fs ⇒
      app (p:'ffi ffi_proj) TextIO_openIn_v [sv]
@@ -824,24 +655,18 @@ Theorem openIn_spec:
        (POSTve
           (\fdv. &(INSTREAM (nextFD fs) fdv ∧
                   validFD (nextFD fs) (openFileFS s fs ReadMode 0) ∧
-                  inFS_fname fs s) *
+                  inFS_fname fs (File s)) *
                 IOFS (openFileFS s fs ReadMode 0))
-
-          (\e. &(BadFileName_exn e ∧ ~inFS_fname fs s) * IOFS fs))
-Proof
-  rw [] >> qpat_abbrev_tac `Q = POSTve _ _` >>
-  simp [IOFS_def, fs_ffi_part_def, IOx_def, IO_def] >>
-  xpull >> qunabbrev_tac `Q` >>
-  xcf_with_def "TextIO.openIn" TextIO_openIn_v_def >>
+          (\e. &(BadFileName_exn e ∧ ~inFS_fname fs (File s)) * IOFS fs))`
+  (xcf_with_def "TextIO.openIn" TextIO_openIn_v_def >>
   fs[FILENAME_def, strlen_def, IOFS_def, IOFS_iobuff_def] >>
-  REVERSE (Cases_on`consistentFS fs`) >-(xpull >> fs[wfFS_def]) >>
   xpull >> rename [`W8ARRAY _ fnm0`] >>
-  qmatch_goalsub_abbrev_tac`catfs fs * _` >>
+  qmatch_goalsub_abbrev_tac`catfs fs` >>
   rpt(xlet_auto >- xsimpl) >>
   qmatch_goalsub_abbrev_tac`W8ARRAY _ fd0` >>
   qmatch_goalsub_rename_tac`W8ARRAY loc fd0` >>
   qmatch_goalsub_abbrev_tac`catfs fs' * _` >>
-  Cases_on `inFS_fname fs s`
+  Cases_on `inFS_fname fs (File s)`
   >- (xlet `POSTv u2.
             &(UNIT_TYPE () u2 /\ nextFD fs < fs.maxFD /\
               validFD (nextFD fs) (openFileFS s fs ReadMode 0)) *
@@ -852,22 +677,23 @@ Proof
         xffi >> xsimpl >>
         qexists_tac`(MAP (n2w o ORD) (explode s) ++ [0w])` >>
         fs[strcat_thm,implode_def] >>
-        simp[fsFFITheory.fs_ffi_part_def,IOx_def,IO_def] >>
-        qmatch_goalsub_abbrev_tac `FFI_part st f ns` >>
+        simp[fsFFITheory.fs_ffi_part_def,IOx_def] >>
+        qmatch_goalsub_abbrev_tac`IO st f ns` >>
         CONV_TAC(RESORT_EXISTS_CONV List.rev) >>
-        map_every qexists_tac[`events`,`ns`,`f`,`st`]
+        map_every qexists_tac[`ns`,`f`,`st`]
         >> xsimpl >>
         simp[Abbr`f`,Abbr`st`,Abbr`ns`, mk_ffi_next_def,
              ffi_open_in_def, (* decode_encode_FS, *) Abbr`fd0`,
              getNullTermStr_add_null, MEM_MAP, ORD_BOUND, ORD_eq_0,
              dimword_8, MAP_MAP_o, o_DEF, char_BIJ,str_def,strcat_thm,
              LENGTH_explode,REPLICATE_compute,LUPDATE_compute,explode_implode] >>
-        imp_res_tac inFS_fname_ALOOKUP_EXISTS >>
+        `∃content. ALOOKUP fs.files (File s) = SOME content`
+          by (fs[inFS_fname_def, ALOOKUP_EXISTS_IFF, MEM_MAP, EXISTS_PROD] >>
+              metis_tac[]) >>
+             (* fs[DROP_LENGTH_TOO_LONG,LENGTH_REPLICATE] *)
         imp_res_tac nextFD_ltX >>
         csimp[openFileFS_def, openFile_def, validFD_def] >>
-        fs[STRING_TYPE_def] \\ xsimpl >>
-        qpat_abbrev_tac `new_events = events ++ _` >>
-        qexists_tac `new_events` >> xsimpl) >>
+        fs[STRING_TYPE_def] \\ xsimpl) >>
     xlet_auto >- xsimpl >>
     xlet_auto >- xsimpl >>
     xlet_auto >- (xsimpl >> imp_res_tac WORD_UNICITY_R >> fs[])
@@ -883,10 +709,10 @@ Proof
             &UNIT_TYPE () u2 * catfs fs * W8ARRAY iobuff_loc fnm0 *
             W8ARRAY loc (LUPDATE 1w 0 fd0)`
   >- (simp[Abbr`catfs`,Abbr`fs'`] >> xffi >> xsimpl >>
-      simp[fsFFITheory.fs_ffi_part_def,IOx_def,IO_def] >>
-      qmatch_goalsub_abbrev_tac `FFI_part st f ns` >>
+      simp[fsFFITheory.fs_ffi_part_def,IOx_def] >>
+      qmatch_goalsub_abbrev_tac`IO st f ns` >>
       CONV_TAC(RESORT_EXISTS_CONV List.rev) >>
-      map_every qexists_tac[`events`,`ns`,`f`,`st`] >> xsimpl >>
+      map_every qexists_tac[`ns`,`f`,`st`] >> xsimpl >>
       qexists_tac`(MAP (n2w o ORD) (explode s) ++ [0w])` >>
       fs[strcat_thm,implode_def] >>
       simp[Abbr`f`,Abbr`st`,Abbr`ns`, mk_ffi_next_def,
@@ -894,20 +720,17 @@ Proof
            getNullTermStr_add_null, MEM_MAP, ORD_BOUND, ORD_eq_0,
            dimword_8, MAP_MAP_o, o_DEF, char_BIJ,str_def,strcat_thm,
            implode_explode, LENGTH_explode] >>
-      fs[not_inFS_fname_openFile,STRING_TYPE_def] \\ xsimpl >>
-      qpat_abbrev_tac `new_events = events ++ _` >>
-      qexists_tac `new_events` >> xsimpl) >>
+      fs[not_inFS_fname_openFile,STRING_TYPE_def] \\ xsimpl) >>
   xlet_auto >-(xsimpl) >> fs[] >>
   xlet_auto >- xsimpl >>
   xlet_auto >- (xsimpl >> imp_res_tac WORD_UNICITY_R) >>
   xif >-(rfs[Abbr`fd0`,EL_LUPDATE,HD_LUPDATE]) >>
   xlet_auto >-(xcon >> xsimpl) >> xraise >> xsimpl >>
-  simp[BadFileName_exn_def,Abbr`fd0`,LENGTH_explode]
-QED
+  simp[BadFileName_exn_def,Abbr`fd0`,LENGTH_explode]);
 
 (* STDIO version *)
-Theorem openIn_STDIO_spec:
-   ∀s sv fs.
+Theorem openIn_STDIO_spec
+  `∀s sv fs.
      FILENAME s sv ∧
      hasFreeFD fs ⇒
      app (p:'ffi ffi_proj) TextIO_openIn_v [sv]
@@ -915,47 +738,41 @@ Theorem openIn_STDIO_spec:
        (POSTve
           (\fdv. &(INSTREAM (nextFD fs) fdv ∧
                   validFD (nextFD fs) (openFileFS s fs ReadMode 0) ∧
-                  inFS_fname fs s) *
+                  inFS_fname fs (File s)) *
                 STDIO (openFileFS s fs ReadMode 0))
-          (\e. &(BadFileName_exn e ∧ ~inFS_fname fs s) * STDIO fs))
-Proof
- rw[STDIO_def] >> xpull >> xapp_spec openIn_spec >>
+          (\e. &(BadFileName_exn e ∧ ~inFS_fname fs (File s)) * STDIO fs))`
+ (rw[STDIO_def] >> xpull >> xapp_spec openIn_spec >>
  map_every qexists_tac [`emp`,`s`,`fs with numchars := ll`] >>
  xsimpl >> rw[] >> qexists_tac`ll` >> fs[openFileFS_fupd_numchars] >> xsimpl >>
  rw[] >>
  fs[nextFD_numchars,nextFD_numchars,openFileFS_fupd_numchars,STD_streams_openFileFS] >>
- fs[GSYM validFD_numchars,GSYM openFileFS_fupd_numchars,inFS_fname_numchars]
-QED
+ fs[GSYM validFD_numchars,GSYM openFileFS_fupd_numchars,inFS_fname_numchars])
 
 (* openOut, openAppend here *)
 
-Theorem closeIn_spec:
-   ∀fdw fdv fs.
+Theorem closeIn_spec
+  `∀fdw fdv fs.
      INSTREAM fdw fdv ⇒
      app (p:'ffi ffi_proj) TextIO_closeIn_v [fdv]
        (IOFS fs)
        (POSTve
           (\u. &(UNIT_TYPE () u /\ validFileFD fdw fs.infds) *
-               IOFS (fs with infds updated_by ADELKEY fdw))
-          (\e. &(InvalidFD_exn e /\ ¬ validFileFD fdw fs.infds) * IOFS fs))
-Proof
-  rw [] >> qpat_abbrev_tac `Q = POSTve _ _` >>
-  simp [IOFS_def, fs_ffi_part_def, IOx_def, IO_def] >>
-  xpull >> qunabbrev_tac `Q` >>
-  xcf_with_def "TextIO.closeIn" TextIO_closeIn_v_def >>
+               IOFS (fs with infds updated_by A_DELKEY fdw))
+          (\e. &(InvalidFD_exn e /\ ¬ validFileFD fdw fs.infds) * IOFS fs))`
+  (xcf_with_def "TextIO.closeIn" TextIO_closeIn_v_def >>
   fs[IOFS_def, IOFS_iobuff_def,INSTREAM_def] >> xpull >>
   rename [`W8ARRAY _ buf`] >> cases_on`buf` >> fs[LUPDATE_def] >>
   xlet_auto >- xsimpl >> fs [get_in_def] >>
   xlet`POSTv uv. &(UNIT_TYPE () uv) *
         W8ARRAY iobuff_loc ((if validFileFD fdw fs.infds then 0w else 1w) ::t) *
         IOx fs_ffi_part (if validFileFD fdw fs.infds then
-                            (fs with infds updated_by ADELKEY fdw)
+                            (fs with infds updated_by A_DELKEY fdw)
                          else fs)`
-  >-(xffi >> simp[IOFS_def,fsFFITheory.fs_ffi_part_def,IOx_def,IO_def] >>
-     qmatch_goalsub_abbrev_tac`FFI_part st f ns` >> xsimpl >>
-     qmatch_goalsub_abbrev_tac`FFI_part (_ fs') f ns` >>
+  >-(xffi >> simp[IOFS_def,fsFFITheory.fs_ffi_part_def,IOx_def] >>
+     qmatch_goalsub_abbrev_tac`IO st f ns` >> xsimpl >>
+     qmatch_goalsub_abbrev_tac`IO (_ fs') f ns` >>
      CONV_TAC(RESORT_EXISTS_CONV List.rev) >>
-     map_every qexists_tac[`events`,`ns`,`f`,`st`] >> xsimpl >>
+     map_every qexists_tac[`ns`,`f`,`st`] >> xsimpl >>
      qexists_tac`n2w8 fdw` >> fs[FD_def] >>
      unabbrev_all_tac >>
      simp[validFileFD_def] >>
@@ -967,43 +784,36 @@ Proof
         implode_explode, LENGTH_explode,closeFD_def,LUPDATE_def] >>
      cases_on`fs` >> fs[IO_fs_infds_fupd] >>
      imp_res_tac ALOOKUP_NONE >> rw[] \\
-     fs[liveFS_def,IO_fs_infds_fupd,STRING_TYPE_def] \\ xsimpl >>
-     qpat_abbrev_tac `new_events = events ++ _` >>
-     qexists_tac `new_events` >> xsimpl) >>
+     fs[liveFS_def,IO_fs_infds_fupd,STRING_TYPE_def] \\ xsimpl) >>
   NTAC 3 (xlet_auto >- xsimpl) >>
   CASE_TAC >> xif >> instantiate
   >-(xcon >> fs[IOFS_def,liveFS_def] >> xsimpl) >>
   xlet_auto >-(xcon >> xsimpl) >>
-  xraise >> fs[InvalidFD_exn_def,IOFS_def] >> xsimpl
-QED
+  xraise >> fs[InvalidFD_exn_def,IOFS_def] >> xsimpl);
 
-Theorem closeOut_spec:
-   ∀fdw fdv fs.
+Theorem closeOut_spec
+  `∀fdw fdv fs.
      OUTSTREAM fdw fdv ⇒
      app (p:'ffi ffi_proj) TextIO_closeOut_v [fdv]
        (IOFS fs)
        (POSTve
          (\u. &(UNIT_TYPE () u /\ validFileFD fdw fs.infds) *
-              IOFS (fs with infds updated_by ADELKEY fdw))
-         (\e. &(InvalidFD_exn e /\ ¬ validFileFD fdw fs.infds) * IOFS fs))
-Proof
-  rw [] >> qpat_abbrev_tac `Q = POSTve _ _` >>
-  simp [IOFS_def, fs_ffi_part_def, IOx_def, IO_def] >>
-  xpull >> qunabbrev_tac `Q` >>
-  xcf_with_def "TextIO.closeOut" TextIO_closeOut_v_def >>
+              IOFS (fs with infds updated_by A_DELKEY fdw))
+         (\e. &(InvalidFD_exn e /\ ¬ validFileFD fdw fs.infds) * IOFS fs))`
+  (xcf_with_def "TextIO.closeOut" TextIO_closeOut_v_def >>
   fs[IOFS_def, IOFS_iobuff_def,OUTSTREAM_def] >> xpull >>
   rename [`W8ARRAY _ buf`] >> cases_on`buf` >> fs[LUPDATE_def] >>
   xlet_auto >- xsimpl >> fs [get_out_def] >>
   xlet`POSTv uv. &(UNIT_TYPE () uv) *
         W8ARRAY iobuff_loc ((if validFileFD fdw fs.infds then 0w else 1w) ::t) *
         IOx fs_ffi_part (if validFileFD fdw fs.infds then
-                            (fs with infds updated_by ADELKEY fdw)
+                            (fs with infds updated_by A_DELKEY fdw)
                          else fs)`
-  >-(xffi >> simp[IOFS_def,fsFFITheory.fs_ffi_part_def,IOx_def,IO_def] >>
-     qmatch_goalsub_abbrev_tac `FFI_part st f ns` >> xsimpl >>
-     qmatch_goalsub_abbrev_tac `FFI_part (_ fs') f ns` >>
+  >-(xffi >> simp[IOFS_def,fsFFITheory.fs_ffi_part_def,IOx_def] >>
+     qmatch_goalsub_abbrev_tac`IO st f ns` >> xsimpl >>
+     qmatch_goalsub_abbrev_tac`IO (_ fs') f ns` >>
      CONV_TAC(RESORT_EXISTS_CONV List.rev) >>
-     map_every qexists_tac[`events`,`ns`,`f`,`st`] >> xsimpl >>
+     map_every qexists_tac[`ns`,`f`,`st`] >> xsimpl >>
      qexists_tac`n2w8 fdw` >> fs[FD_def] >>
      unabbrev_all_tac >>
      simp[validFileFD_def] >>
@@ -1015,58 +825,51 @@ Proof
         implode_explode, LENGTH_explode,closeFD_def,LUPDATE_def] >>
      cases_on`fs` >> fs[IO_fs_infds_fupd] >>
      imp_res_tac ALOOKUP_NONE >> rw[] \\
-     fs[liveFS_def,IO_fs_infds_fupd,STRING_TYPE_def] \\ xsimpl >>
-     qpat_abbrev_tac `new_events = events ++ _` >>
-     qexists_tac `new_events` >> xsimpl) >>
+     fs[liveFS_def,IO_fs_infds_fupd,STRING_TYPE_def] \\ xsimpl) >>
   NTAC 3 (xlet_auto >- xsimpl) >>
   CASE_TAC >> xif >> instantiate
   >-(xcon >> fs[IOFS_def,liveFS_def] >> xsimpl) >>
   xlet_auto >-(xcon >> xsimpl) >>
-  xraise >> fs[InvalidFD_exn_def,IOFS_def] >> xsimpl
-QED
+  xraise >> fs[InvalidFD_exn_def,IOFS_def] >> xsimpl);
 
-Theorem closeIn_STDIO_spec:
-   ∀fd fs fdv.
+Theorem closeIn_STDIO_spec
+  `∀fd fs fdv.
      INSTREAM fd fdv /\ fd >= 3 /\ fd <= fs.maxFD ⇒
      app (p:'ffi ffi_proj) TextIO_closeIn_v [fdv]
        (STDIO fs)
        (POSTve
           (\u. &(UNIT_TYPE () u /\ validFileFD fd fs.infds) *
-               STDIO (fs with infds updated_by ADELKEY fd))
-          (\e. &(InvalidFD_exn e /\ ¬ validFileFD fd fs.infds) * STDIO fs))
-Proof
-  rw[STDIO_def] >> xpull >> xapp_spec closeIn_spec >>
+               STDIO (fs with infds updated_by A_DELKEY fd))
+          (\e. &(InvalidFD_exn e /\ ¬ validFileFD fd fs.infds) * STDIO fs))`
+  (rw[STDIO_def] >> xpull >> xapp_spec closeIn_spec >>
   map_every qexists_tac [`emp`,`fs with numchars := ll`,`fd`] >>
   xsimpl >> rw[] >> qexists_tac`ll` >> fs[validFileFD_def] >> xsimpl >>
   fs[STD_streams_def,ALOOKUP_ADELKEY] \\
   Cases_on`fd = 0` \\ fs[]
   \\ Cases_on`fd = 1` \\ fs[]
   \\ Cases_on`fd = 2` \\ fs[]
-  \\ metis_tac[]
-QED
+  \\ metis_tac[]);
 
-Theorem closeOut_STDIO_spec:
-   ∀fd fs fdv.
+Theorem closeOut_STDIO_spec
+  `∀fd fs fdv.
      OUTSTREAM fd fdv /\ fd >= 3 /\ fd <= fs.maxFD ⇒
      app (p:'ffi ffi_proj) TextIO_closeOut_v [fdv]
        (STDIO fs)
        (POSTve
           (\u. &(UNIT_TYPE () u /\ validFileFD fd fs.infds) *
-               STDIO (fs with infds updated_by ADELKEY fd))
-          (\e. &(InvalidFD_exn e /\ ¬ validFileFD fd fs.infds) * STDIO fs))
-Proof
-  rw[STDIO_def] >> xpull >> xapp_spec closeOut_spec >>
+               STDIO (fs with infds updated_by A_DELKEY fd))
+          (\e. &(InvalidFD_exn e /\ ¬ validFileFD fd fs.infds) * STDIO fs))`
+  (rw[STDIO_def] >> xpull >> xapp_spec closeOut_spec >>
   map_every qexists_tac [`emp`,`fs with numchars := ll`,`fd`] >>
   xsimpl >> rw[] >> qexists_tac`ll` >> fs[validFileFD_def] >> xsimpl >>
   fs[STD_streams_def,ALOOKUP_ADELKEY] \\
   Cases_on`fd = 0` \\ fs[]
   \\ Cases_on`fd = 1` \\ fs[]
   \\ Cases_on`fd = 2` \\ fs[]
-  \\ metis_tac[]
-QED
+  \\ metis_tac[]);
 
-Theorem writei_spec:
-  wfFS fs ⇒ 0 < n ⇒
+Theorem writei_spec
+ `wfFS fs ⇒ 0 < n ⇒
    MAX (i+n) 2048 <= LENGTH rest ⇒ i + n < 256**2 ⇒
   get_file_content fs fd = SOME(content, pos) ⇒
   get_mode fs fd = SOME WriteMode ⇒
@@ -1082,9 +885,8 @@ Theorem writei_spec:
                   (insert_atI (TAKE nw (MAP (CHR o w2n) (DROP i rest))) pos
                                     content)))
     (\e. &(InvalidFD_exn e) * W8ARRAY iobuff_loc (1w :: n2w n :: n2w2 i ++ rest) * &(F) *
-         IOFS (fs with numchars:= THE(LDROP (1 + Lnext_pos fs.numchars) fs.numchars))))
-Proof
-  strip_tac >>
+         IOFS (fs with numchars:= THE(LDROP (1 + Lnext_pos fs.numchars) fs.numchars))))`
+  (strip_tac >>
   `?ll. fs.numchars = ll` by simp[]  >> fs[] >>
   `ll ≠ [||]`  by (cases_on`ll` >> fs[wfFS_def,liveFS_def,live_numchars_def]) >>
   `always (eventually (λll. ∃k. LHD ll = SOME k ∧ k ≠ 0)) ll`
@@ -1108,16 +910,12 @@ Proof
                           (TAKE pos content ++
                            TAKE (MIN n k) (MAP (CHR o w2n) (DROP i rest)) ++
                            DROP (MIN n k + pos) content))`
-     >-(qmatch_goalsub_abbrev_tac` _ * _ * IOx _ fs'` >>
-        qpat_abbrev_tac `Q = $POSTv _` >>
-        simp [fs_ffi_part_def, IOx_def, IO_def] >>
-        xpull >> qunabbrev_tac `Q` >>
-        xffi >> xsimpl >>
+     >-(qmatch_goalsub_abbrev_tac` _ * _ * IOx _ fs'` >> xffi >> xsimpl >>
         fs[IOFS_def,IOx_def,fs_ffi_part_def,
-               mk_ffi_next_def, IO_def] >>
-        qmatch_goalsub_abbrev_tac `FFI_part st f ns` >>
+               mk_ffi_next_def] >>
+        qmatch_goalsub_abbrev_tac`IO st f ns` >>
         CONV_TAC(RESORT_EXISTS_CONV List.rev) >>
-        map_every qexists_tac[`events`,`ns`,`f`,`st`] >> xsimpl >>
+        map_every qexists_tac[`ns`,`f`,`st`] >> xsimpl >>
         qexists_tac`n2w8 fd` >>
         fs[Abbr`f`,Abbr`st`,Abbr`ns`,mk_ffi_next_def,w82n_n2w8,LENGTH_n2w8,
            ffi_write_def,(* decode_encode_FS, *)MEM_MAP, ORD_BOUND,ORD_eq_0,wfFS_LDROP,
@@ -1134,9 +932,7 @@ Proof
         rw[] >> rfs[]
         \\ Cases_on`md` \\ fs[]
         >- rfs[get_mode_def]
-        \\ xsimpl \\ simp[n2w2_def] >>
-        qpat_abbrev_tac `new_events = events ++ _` >>
-        qexists_tac `new_events` >> xsimpl) >>
+        \\ xsimpl \\ simp[n2w2_def]) >>
      qmatch_goalsub_abbrev_tac` _ * IOx _ fs'` >>
      qmatch_goalsub_abbrev_tac`W8ARRAY _ (_::m1 :: m0 :: n2w i :: rest)` >>
      fs[] >>
@@ -1156,16 +952,12 @@ Proof
                           (TAKE pos content ++
                            TAKE 0 (MAP (CHR o w2n) (DROP i rest)) ++
                            DROP pos content))`
-  >-(qmatch_goalsub_abbrev_tac` _ * _ * IOx _ fs'` >>
-     qpat_abbrev_tac `Q = $POSTv _` >>
-     simp [fs_ffi_part_def, IOx_def, IO_def] >>
-     xpull >> qunabbrev_tac `Q` >>
-     xffi >> xsimpl >>
+  >-(qmatch_goalsub_abbrev_tac` _ * _ * IOx _ fs'` >> xffi >> xsimpl >>
      fs[IOFS_def,IOx_def,fs_ffi_part_def,
-            mk_ffi_next_def,IO_def] >>
-     qmatch_goalsub_abbrev_tac `FFI_part st f ns` >>
+            mk_ffi_next_def] >>
+     qmatch_goalsub_abbrev_tac`IO st f ns` >>
      CONV_TAC(RESORT_EXISTS_CONV List.rev) >>
-     map_every qexists_tac[`events`,`ns`,`f`,`st`] >> xsimpl >>
+     map_every qexists_tac[`ns`,`f`,`st`] >> xsimpl >>
      qexists_tac`n2w8 fd` >>
      fs[Abbr`f`,Abbr`st`,Abbr`ns`,mk_ffi_next_def,
         ffi_write_def,(* decode_encode_FS, *)MEM_MAP, ORD_BOUND,ORD_eq_0,wfFS_LDROP,
@@ -1182,9 +974,7 @@ Proof
      rw[] >> rfs[]
      \\ Cases_on`md` \\ fs[]
      >- rfs[get_mode_def]
-     \\ xsimpl >>
-     qpat_abbrev_tac `new_events = events ++ _` >>
-     qexists_tac `new_events` >> xsimpl) >>
+     \\ xsimpl) >>
   NTAC 3 (xlet_auto >- xsimpl) >>
   xif >> fs[FALSE_def] >> instantiate >>
   NTAC 2 (xlet_auto >- xsimpl) >>
@@ -1200,20 +990,19 @@ Proof
   sg`fs' = fs with numchars := t`
   >-(imp_res_tac validFD_ALOOKUP >> fs[wfFS_def,Abbr`fs'`,fsupdate_def] >>
      fs[IO_fs_component_equality] >> fs[wfFS_def,get_file_content_def] >>
-     pairarg_tac >> fs[AFUPDKEY_unchanged,LDROP_1]) >>
+     pairarg_tac >> fs[ALIST_FUPDKEY_unchanged,LDROP_1]) >>
   fs[Abbr`fs'`,get_file_content_def,liveFS_def,live_numchars_def,fsupdate_def,LDROP_1,
      wfFS_fsupdate,validFD_def,liveFS_fsupdate,IOFS_def] >>
-  pairarg_tac >> fs[AFUPDKEY_unchanged] >>
+  pairarg_tac >> fs[ALIST_FUPDKEY_unchanged] >>
   fs[wfFS_def,liveFS_def,live_numchars_def] >>
   imp_res_tac always_thm >>
   `Lnext_pos (0:::t) = SUC(Lnext_pos t)` by
     (fs[Lnext_pos_def,Once Lnext_def]) >>
   csimp[ADD] >> xsimpl >> cases_on`t` >>
-  fs[get_mode_def] >> rw[] >> instantiate >> xsimpl
-QED
+  fs[get_mode_def] >> rw[] >> instantiate >> xsimpl);
 
-Theorem write_spec:
-   !n fs fd i pos h1 h2 h3 h4 rest bc fdv nv iv content.
+Theorem write_spec
+  `!n fs fd i pos h1 h2 h3 h4 rest bc fdv nv iv content.
    wfFS fs ⇒ MAX(i + n) 2048 <= LENGTH rest ⇒ i + n < 256 ** 2 ⇒
    get_file_content fs fd = SOME(content, pos) ⇒
    get_mode fs fd = SOME WriteMode ⇒
@@ -1224,9 +1013,8 @@ Theorem write_spec:
    (POSTv nwv. SEP_EXISTS k.
       IOFS(fsupdate fs fd k (pos + n)
                     (insert_atI (TAKE n (MAP (CHR o w2n) (DROP i rest))) pos
-                                     content)))
-Proof
-  strip_tac >> `?N. n <= N` by (qexists_tac`n` >> fs[]) >>
+                                     content)))`
+  (strip_tac >> `?N. n <= N` by (qexists_tac`n` >> fs[]) >>
   FIRST_X_ASSUM MP_TAC >> qid_spec_tac`n` >>
   Induct_on`N` >>
   xcf_with_def "TextIO.write" TextIO_write_v_def
@@ -1240,7 +1028,7 @@ Proof
   >-(xcon >> xsimpl >> fs[IOFS_def,IOFS_iobuff_def] >> xsimpl >>
          qexists_tac`(Lnext_pos fs.numchars + 1)` >> `nw = n` by fs[] >> xsimpl >>
      imp_res_tac get_file_content_validFD >>
-     fs[wfFS_fsupdate,validFD_def,always_DROP,AFUPDKEY_ALOOKUP,
+     fs[wfFS_fsupdate,validFD_def,always_DROP,ALIST_FUPDKEY_ALOOKUP,
         liveFS_fsupdate,get_file_content_def,LENGTH_n2w2]) >>
   NTAC 2 (xlet_auto >- xsimpl) >>
   qmatch_goalsub_abbrev_tac`IOx _ fs'` >>
@@ -1252,8 +1040,8 @@ Proof
   NTAC 3 (strip_tac >-(
       imp_res_tac get_file_content_validFD >>
                   fs[Abbr`fs'`,liveFS_def,live_numchars_def,LDROP_1, wfFS_fsupdate,validFD_def,
-                         always_DROP,AFUPDKEY_ALOOKUP,get_file_content_def,get_mode_def] >>
-                  pairarg_tac >> fs[fsupdate_def,always_DROP,AFUPDKEY_ALOOKUP] >>
+                         always_DROP,ALIST_FUPDKEY_ALOOKUP,get_file_content_def,get_mode_def] >>
+                  pairarg_tac >> fs[fsupdate_def,always_DROP,ALIST_FUPDKEY_ALOOKUP] >>
           imp_res_tac NOT_LFINITE_DROP >>
           FIRST_X_ASSUM (ASSUME_TAC o Q.SPEC`(Lnext_pos fs.numchars + 1)`) >>
           fs[] >> imp_res_tac NOT_LFINITE_DROP_LFINITE)) >>
@@ -1262,11 +1050,10 @@ Proof
   qmatch_abbrev_tac`_ (_ _ _ _ _ (_ c1 _ _)) ==>> _ (_ _ _ _ _ (_ c2 _ _)) * _` >>
   `c1 = c2` suffices_by xsimpl >> fs[Abbr`c1`,Abbr`c2`] >>
   PURE_REWRITE_TAC[Once (Q.SPECL [`i`,`nw`] ADD_COMM)] >>
-  fs[Once ADD_COMM,GSYM DROP_DROP_T,take_drop_partition,MAP_DROP]
-QED
+  fs[Once ADD_COMM,GSYM DROP_DROP_T,take_drop_partition,MAP_DROP]);
 
-Theorem output1_spec:
-   !fd fdv c cv bc content pos.
+Theorem output1_spec
+  `!fd fdv c cv bc content pos.
     get_file_content fs fd = SOME(content, pos) ⇒
     get_mode fs fd = SOME WriteMode ⇒
     CHAR c cv ⇒ OUTSTREAM fd fdv ⇒
@@ -1274,9 +1061,8 @@ Theorem output1_spec:
     (IOFS fs)
     (POSTv uv.
       &UNIT_TYPE () uv * SEP_EXISTS k.
-      IOFS (fsupdate fs fd k (pos+1) (insert_atI [c] pos content)))
-Proof
-  xcf_with_def "TextIO.output1" TextIO_output1_v_def >>
+      IOFS (fsupdate fs fd k (pos+1) (insert_atI [c] pos content)))`
+  (xcf_with_def "TextIO.output1" TextIO_output1_v_def >>
   fs[IOFS_def,IOFS_iobuff_def] >>
   xpull >> rename [`W8ARRAY _ bdef`] >>
   ntac 3 (xlet_auto >- xsimpl) >>
@@ -1290,20 +1076,18 @@ Proof
   simp[LUPDATE_compute] >>
   xlet_auto >-(xsimpl >> fs [FD_def]) >>
   xcon >> fs[IOFS_def,IOFS_iobuff_def] >> xsimpl >> rw[] >>
-  fs[CHR_ORD,LESS_MOD,ORD_BOUND] >> qexists_tac`k` >> xsimpl
-QED
+  fs[CHR_ORD,LESS_MOD,ORD_BOUND] >> qexists_tac`k` >> xsimpl);
 
-Theorem output1_STDIO_spec:
-   !fd. get_file_content fs fd = SOME(content, pos) ∧
+Theorem output1_STDIO_spec
+  `!fd. get_file_content fs fd = SOME(content, pos) ∧
         get_mode fs fd = SOME WriteMode ∧
    CHAR c cv ∧ OUTSTREAM fd fdv ⇒
    app (p:'ffi ffi_proj) TextIO_output1_v [fdv; cv]
    (STDIO fs)
    (POSTv uv.
      &UNIT_TYPE () uv *
-     STDIO (fsupdate fs fd 0 (pos+1) (insert_atI [c] pos content)))
-Proof
-  rw[STDIO_def] \\ xpull \\ xapp_spec output1_spec \\
+     STDIO (fsupdate fs fd 0 (pos+1) (insert_atI [c] pos content)))`
+  (rw[STDIO_def] \\ xpull \\ xapp_spec output1_spec \\
   mp_tac(SYM(SPEC_ALL get_file_content_numchars)) \\ rw[] \\
   mp_tac(get_mode_with_numchars) \\ rw[] \\
   instantiate \\ simp[GSYM validFD_numchars] \\ xsimpl \\ rw[] \\
@@ -1319,8 +1103,7 @@ Proof
   \\ qmatch_abbrev_tac`IOFS fs1 ==>> IOFS fs2 * _`
   \\ `fs1 = fs2` suffices_by xsimpl
   \\ fs[get_file_content_def] \\ pairarg_tac \\ fs[]
-  \\ rw[Abbr`fs1`,Abbr`fs2`,IO_fs_component_equality,fsupdate_def]
-QED
+  \\ rw[Abbr`fs1`,Abbr`fs2`,IO_fs_component_equality,fsupdate_def]);
 
 val tac =
      simp[w82n_n2w8,FD_def,LENGTH_n2w8,STRING_TYPE_def] \\ xsimpl
@@ -1335,32 +1118,28 @@ val tac =
   \\ simp[Q.ISPEC`explode x`(Q.GEN`l2`insert_atI_end) |> SIMP_RULE(srw_ss())[]]
   \\ xsimpl;
 
-Theorem output1_stdout_spec:
-   CHAR c cv ∧ fdv = stdout_v ==>
+Theorem output1_stdout_spec
+  `CHAR c cv ∧ fdv = stdout_v ==>
    app (p:'ffi ffi_proj) TextIO_output1_v
      [fdv; cv] (STDIO fs)
-     (POSTv uv. &UNIT_TYPE () uv * STDIO (add_stdout fs (str c)))
-Proof
-  reverse(Cases_on`STD_streams fs`) >- (fs[STDIO_def] \\ strip_tac \\ xpull)
+     (POSTv uv. &UNIT_TYPE () uv * STDIO (add_stdout fs (str c)))`
+  (reverse(Cases_on`STD_streams fs`) >- (fs[STDIO_def] \\ strip_tac \\ xpull)
   \\ strip_tac
   \\ xapp_spec output1_STDIO_spec
-  \\ tac
-QED
+  \\ tac);
 
-Theorem output1_stderr_spec:
-   CHAR c cv ∧ fdv = stderr_v ==>
+Theorem output1_stderr_spec
+  `CHAR c cv ∧ fdv = stderr_v ==>
    app (p:'ffi ffi_proj) TextIO_output1_v
      [fdv; cv] (STDIO fs)
-     (POSTv uv. &UNIT_TYPE () uv * STDIO (add_stderr fs (str c)))
-Proof
-  reverse(Cases_on`STD_streams fs`) >- (fs[STDIO_def] \\ strip_tac \\ xpull)
+     (POSTv uv. &UNIT_TYPE () uv * STDIO (add_stderr fs (str c)))`
+  (reverse(Cases_on`STD_streams fs`) >- (fs[STDIO_def] \\ strip_tac \\ xpull)
   \\ strip_tac
   \\ xapp_spec output1_STDIO_spec
-  \\ tac
-QED
+  \\ tac);
 
-Theorem output_spec:
-   !s fd fdv sv fs content pos.
+Theorem output_spec
+  `!s fd fdv sv fs content pos.
     OUTSTREAM fd fdv ⇒ STRING_TYPE s sv ⇒
     (get_file_content fs fd = SOME(content, pos)) ⇒
     (get_mode fs fd = SOME WriteMode) ⇒
@@ -1368,9 +1147,8 @@ Theorem output_spec:
     (IOFS fs)
     (POSTv uv. &(UNIT_TYPE () uv) *
        SEP_EXISTS k. IOFS (fsupdate fs fd k (pos + (strlen s))
-                                    (insert_atI (explode s) pos content)))
-Proof
-  strip_tac >>
+                                    (insert_atI (explode s) pos content)))`
+  (strip_tac >>
   `?n. strlen s <= n` by (qexists_tac`strlen s` >> fs[]) >>
   FIRST_X_ASSUM MP_TAC >> qid_spec_tac`s` >>
   Induct_on`n` >>
@@ -1415,7 +1193,7 @@ Proof
   fs[get_file_content_def, get_mode_def] >> pairarg_tac >>
   fs[Abbr`fs'`,Abbr`pos'`,Abbr`content'`,liveFS_def,live_numchars_def,
      fsupdate_def,LDROP_1, wfFS_fsupdate,validFD_def,always_DROP,
-     AFUPDKEY_ALOOKUP,extract_def,strlen_extract_le,
+     ALIST_FUPDKEY_ALOOKUP,extract_def,strlen_extract_le,
      MIN_DEF] >> xsimpl >>
   rpt strip_tac >>
   qexists_tac`x' + k` >> fs[insert_atI_def] >>
@@ -1428,11 +1206,11 @@ Proof
       CASE_TAC \\ fs[] \\
       imp_res_tac LDROP_NONE_LFINITE
       \\ fs[wfFS_def,liveFS_def,live_numchars_def] ) >>
-    fs[AFUPDKEY_o] >>
-    match_mp_tac AFUPDKEY_eq >>
+    fs[ALIST_FUPDKEY_o] >>
+    match_mp_tac ALIST_FUPDKEY_eq >>
     fs[PAIR_MAP_THM,FORALL_PROD] ) >>
-  fs[AFUPDKEY_o] >>
-  match_mp_tac AFUPDKEY_eq >>
+  fs[ALIST_FUPDKEY_o] >>
+  match_mp_tac ALIST_FUPDKEY_eq >>
   simp[] >>
   fs[MAP_MAP_o,CHR_w2n_n2w_ORD] >>
   IF_CASES_TAC >-
@@ -1444,18 +1222,16 @@ Proof
   IF_CASES_TAC \\
   fs[TAKE_LENGTH_ID_rwt,LENGTH_explode,strlen_substring,
      DROP_DROP_T,TAKE_LENGTH_TOO_LONG,DROP_LENGTH_TOO_LONG]
-  \\ Cases_on`s` \\ fs[substring_def,SEG_TAKE_DROP,TAKE_LENGTH_ID_rwt]
-QED
+  \\ Cases_on`s` \\ fs[substring_def,SEG_TAKE_DROP,TAKE_LENGTH_ID_rwt]);
 
-Theorem output_STDIO_spec:
-   !fd fdv fs content pos s.
+Theorem output_STDIO_spec
+  `!fd fdv fs content pos s.
    OUTSTREAM fd fdv ∧ get_file_content fs fd = SOME (content,pos) ∧ get_mode fs fd = SOME WriteMode ∧ STRING_TYPE s sv ⇒
    app (p:'ffi ffi_proj) TextIO_output_v [fdv;sv]
    (STDIO fs)
    (POSTv uv. &(UNIT_TYPE () uv) *
-      STDIO (fsupdate fs fd 0 (pos+strlen s) (insert_atI (explode s) pos content)))
-Proof
-  rpt strip_tac
+      STDIO (fsupdate fs fd 0 (pos+strlen s) (insert_atI (explode s) pos content)))`
+  (rpt strip_tac
   \\ fs[STDIO_def]
   \\ xpull
   \\ xapp_spec output_spec
@@ -1474,86 +1250,81 @@ Proof
   by (
     fs[STD_streams_def]
     \\ metis_tac[SOME_11,PAIR,FST,SND] ) \\
-  rw[] \\ fs[] \\ simp[insert_atI_end,LENGTH_explode]
-QED
+  rw[] \\ fs[] \\ simp[insert_atI_end,LENGTH_explode]);
 
-Theorem print_spec:
-   !fs sv s.
+Theorem print_spec
+  `!fs sv s.
     STRING_TYPE s sv ⇒
     app (p:'ffi ffi_proj) TextIO_print_v [sv]
     (STDIO fs)
-    (POSTv uv. &(UNIT_TYPE () uv) * STDIO (add_stdout fs s))
-Proof
-  xcf_with_def "TextIO.print" TextIO_print_v_def
+    (POSTv uv. &(UNIT_TYPE () uv) * STDIO (add_stdout fs s))`
+  (xcf_with_def "TextIO.print" TextIO_print_v_def
   \\ reverse(Cases_on`STD_streams fs`) >- (fs[STDIO_def] \\ xpull)
   \\ xapp_spec output_STDIO_spec
-  \\ tac
-QED
+  \\ tac);
 
 val print_def = Define `
   print s = (\fs. (Success (), add_stdout fs s))`
 
-Theorem EvalM_print:
-   Eval env exp (STRING_TYPE x) /\
+Theorem EvalM_print
+  `Eval env exp (STRING_TYPE x) /\
    (nsLookup env.v (Short "print") = SOME TextIO_print_v) ==>
     EvalM F env st (App Opapp [Var (Short "print"); exp])
       (MONAD UNIT_TYPE exc_ty (print x))
-      (MONAD_IO,p:'ffi ffi_proj)
-Proof
-    ho_match_mp_tac EvalM_from_app \\ rw [print_def]
-    \\ fs [MONAD_IO_def]
-    \\ xpull
-    \\ fs [SEP_CLAUSES]
-    \\ xapp_spec print_spec
-    \\ fs[]
-QED
+      (MONAD_IO,p:'ffi ffi_proj)`
+  (ho_match_mp_tac EvalM_from_app \\ rw [print_def]
+  \\ fs [MONAD_IO_def]
+  \\ xpull
+  \\ fs [SEP_CLAUSES]
+  \\ match_mp_tac (app_weaken |> SIMP_RULE (srw_ss()) [AND_IMP_INTRO])
+  \\ drule (GEN_ALL print_spec)
+  \\ disch_then (qspecl_then [`p`,`s`] assume_tac)
+  \\ asm_exists_tac \\ fs []
+  \\ xsimpl);
 
-Theorem output_stderr_spec:
-   !fs sv s fdv.
+Theorem output_stderr_spec
+  `!fs sv s fdv.
     STRING_TYPE s sv ∧ fdv = stderr_v ⇒
     app (p:'ffi ffi_proj) TextIO_output_v [fdv;sv]
     (STDIO fs)
-    (POSTv uv. &(UNIT_TYPE () uv) * STDIO (add_stderr fs s))
-Proof
-  rpt strip_tac
+    (POSTv uv. &(UNIT_TYPE () uv) * STDIO (add_stderr fs s))`
+  (rpt strip_tac
   \\ reverse(Cases_on`STD_streams fs`) >- (fs[STDIO_def] \\ xpull)
   \\ xapp_spec output_STDIO_spec
-  \\ tac
-QED
+  \\ tac);
 
-Theorem print_err_spec:
-   !fs sv s.
+Theorem print_err_spec
+  `!fs sv s.
     STRING_TYPE s sv ⇒
     app (p:'ffi ffi_proj) TextIO_print_err_v [sv]
     (STDIO fs)
-    (POSTv uv. &(UNIT_TYPE () uv) * STDIO (add_stderr fs s))
-Proof
-  xcf_with_def "TextIO.print_err" TextIO_print_err_v_def
+    (POSTv uv. &(UNIT_TYPE () uv) * STDIO (add_stderr fs s))`
+  (xcf_with_def "TextIO.print_err" TextIO_print_err_v_def
   \\ reverse(Cases_on`STD_streams fs`) >- (fs[STDIO_def] \\ xpull)
-  \\ xapp_spec output_stderr_spec \\ fs []
-QED
+  \\ xapp_spec output_stderr_spec \\ fs []);
 
 val print_err_def = Define `
   print_err s = (\fs. (Success (), add_stderr fs s))`;
 
-Theorem EvalM_print_err:
-   Eval env exp (STRING_TYPE x) /\
+Theorem EvalM_print_err
+  `Eval env exp (STRING_TYPE x) /\
     (nsLookup env.v (Long "TextIO" (Short "print_err")) =
       SOME TextIO_print_err_v) ==>
     EvalM F env st (App Opapp [Var (Long "TextIO" (Short "print_err")); exp])
       (MONAD UNIT_TYPE exc_ty (print_err x))
-      (MONAD_IO,p:'ffi ffi_proj)
-Proof
-    ho_match_mp_tac EvalM_from_app \\ rw [print_err_def]
-    \\ fs [MONAD_IO_def]
-    \\ xpull
-    \\ fs [SEP_CLAUSES]
-    \\ xapp_spec print_err_spec
-    \\ fs[]
-QED
+      (MONAD_IO,p:'ffi ffi_proj)`
+  (ho_match_mp_tac EvalM_from_app \\ rw [print_err_def]
+  \\ fs [MONAD_IO_def]
+  \\ xpull
+  \\ fs [SEP_CLAUSES]
+  \\ match_mp_tac (app_weaken |> SIMP_RULE (srw_ss()) [AND_IMP_INTRO])
+  \\ drule (GEN_ALL print_err_spec)
+  \\ disch_then (qspecl_then [`p`,`s`] assume_tac)
+  \\ asm_exists_tac \\ fs []
+  \\ xsimpl);
 
-Theorem read_spec:
-   !fs fd fdv n nv rest h1 h2 h3 h4. wfFS fs ⇒ FD fd fdv ⇒ NUM n nv ⇒
+Theorem read_spec
+  `!fs fd fdv n nv. wfFS fs ⇒ FD fd fdv ⇒ NUM n nv ⇒
    n < 256**2 ⇒ MAX n 2048 <= LENGTH rest ⇒
    app (p:'ffi ffi_proj) TextIO_read_v [fdv;nv]
    (W8ARRAY iobuff_loc (h1::h2::h3::h4::rest) * IOx fs_ffi_part fs)
@@ -1568,22 +1339,18 @@ Theorem read_spec:
       IOx fs_ffi_part (bumpFD fd fs nr) *
       W8ARRAY iobuff_loc (0w :: n2w (nr DIV 256) :: n2w nr :: h4::
         MAP (n2w o ORD) (TAKE nr (DROP pos content))++DROP nr rest))
-     (\e. &InvalidFD_exn e * &(get_file_content fs fd = NONE ∨ get_mode fs fd ≠ SOME ReadMode) * IOFS fs))
-Proof
-   xcf_with_def "TextIO.read" TextIO_read_v_def >>
+     (\e. &InvalidFD_exn e * &(get_file_content fs fd = NONE ∨ get_mode fs fd ≠ SOME ReadMode) * IOFS fs))`
+   (xcf_with_def "TextIO.read" TextIO_read_v_def >>
    fs[IOFS_def,IOFS_iobuff_def] >>
    xlet_auto >- xsimpl >>
    simp[insert_atI_def,n2w2_def] >>
    cases_on`get_file_content fs fd`
    >-(xlet`POSTv v. W8ARRAY iobuff_loc (1w::n2w n::h3::h4::rest) * IOx fs_ffi_part fs`
-      >-(qpat_abbrev_tac `Q = $POSTv _` >>
-         simp [fs_ffi_part_def, IOx_def, IO_def] >>
-         xpull >> qunabbrev_tac `Q` >>
-         xffi >> xsimpl >>
-         fs[IOFS_def,IOx_def,fs_ffi_part_def, mk_ffi_next_def,IO_def] >>
-         qmatch_goalsub_abbrev_tac `FFI_part st f ns` >>
+      >-(xffi >> xsimpl >>
+         fs[IOFS_def,IOx_def,fs_ffi_part_def, mk_ffi_next_def] >>
+         qmatch_goalsub_abbrev_tac`IO st f ns` >>
          CONV_TAC(RESORT_EXISTS_CONV List.rev) >>
-         map_every qexists_tac[`events`,`ns`,`f`, `st`] >>
+         map_every qexists_tac[`ns`,`f`] >>
          xsimpl >> qexists_tac`n2w8 fd` >>
          fs[Abbr`f`,Abbr`st`,Abbr`ns`,mk_ffi_next_def, ffi_read_def,
             w82n_n2w8,LENGTH_n2w8,MEM_MAP, ORD_BOUND,ORD_eq_0,wfFS_LDROP,
@@ -1592,10 +1359,8 @@ Proof
             get_file_content_def,n2w_w2n,w2n_n2w,FD_def,STRING_TYPE_def] >> rfs[] >>
          `n < 2 ** (2 * 8)` by fs[] >> imp_res_tac w22n_n2w2 >>
          fs[n2w2_def] >> xsimpl >>
-         TRY (pairarg_tac >> fs[] >>
-              TRY(Cases_on`md`) >> fs[] >> xsimpl) >>
-         qpat_abbrev_tac `new_events = events ++ _` >>
-         qexists_tac `new_events` >> xsimpl) >>
+         pairarg_tac >> fs[] >>
+         TRY(Cases_on`md`) >> fs[] >> xsimpl) >>
       rpt(xlet_auto >- xsimpl) >> xif >> instantiate >>
       xlet_auto >-(xcon >> xsimpl >> instantiate >> xsimpl) >>
       xraise >> xsimpl >> fs[InvalidFD_exn_def] >> xsimpl) >>
@@ -1604,14 +1369,11 @@ Proof
    >- fs[get_mode_def, get_file_content_def] >>
    reverse(cases_on`x` >> fs[])
    >-(xlet`POSTv v. W8ARRAY iobuff_loc (1w::n2w n::h3::h4::rest) * IOx fs_ffi_part fs`
-      >-(qpat_abbrev_tac `Q = $POSTv _` >>
-         simp [fs_ffi_part_def, IOx_def, IO_def] >>
-         xpull >> qunabbrev_tac `Q` >>
-         xffi >> xsimpl >>
-         fs[IOFS_def,IOx_def,fs_ffi_part_def, mk_ffi_next_def,IO_def] >>
-         qmatch_goalsub_abbrev_tac `FFI_part st f ns` >>
+      >-(xffi >> xsimpl >>
+         fs[IOFS_def,IOx_def,fs_ffi_part_def, mk_ffi_next_def] >>
+         qmatch_goalsub_abbrev_tac`IO st f ns` >>
          CONV_TAC(RESORT_EXISTS_CONV List.rev) >>
-         map_every qexists_tac[`events`,`ns`,`f`,`st`] >>
+         map_every qexists_tac[`ns`,`f`] >>
          xsimpl >> qexists_tac`n2w8 fd` >>
          fs[Abbr`f`,Abbr`st`,Abbr`ns`,mk_ffi_next_def, ffi_read_def,
             w82n_n2w8,LENGTH_n2w8,MEM_MAP, ORD_BOUND,ORD_eq_0,wfFS_LDROP,
@@ -1621,9 +1383,7 @@ Proof
          `n < 2 ** (2 * 8)` by fs[] >> imp_res_tac w22n_n2w2 >>
          rfs[get_mode_def] >>
          fs[n2w2_def] >> xsimpl >>
-         pairarg_tac >> fs[] >> xsimpl >>
-         qpat_abbrev_tac `new_events = events ++ _` >>
-         qexists_tac `new_events` >> xsimpl) >>
+         pairarg_tac >> fs[] >> xsimpl) >>
       rpt(xlet_auto >- xsimpl) >> xif >> instantiate >>
       xlet_auto >-(xcon >> xsimpl >> instantiate >> xsimpl) >>
       xraise >> xsimpl >> fs[InvalidFD_exn_def] >> xsimpl) >>
@@ -1636,14 +1396,11 @@ Proof
         W8ARRAY iobuff_loc (0w :: n2w (nr DIV 256) :: n2w nr :: h4 ::
           (MAP (n2w o ORD) (TAKE nr (DROP pos content))++DROP nr rest)))
           (\e. &(get_file_content fs fd = NONE))` >> xsimpl
-   >-(qpat_abbrev_tac `Q = POSTve _ _` >>
-      simp [fs_ffi_part_def, IOx_def, IO_def] >>
-      xpull >> qunabbrev_tac `Q` >>
-      xffi >> xsimpl >>
-      fs[IOFS_def,IOx_def,fs_ffi_part_def, mk_ffi_next_def,IO_def] >>
-      qmatch_goalsub_abbrev_tac `FFI_part st f ns` >>
+   >-(xffi >> xsimpl >>
+      fs[IOFS_def,IOx_def,fs_ffi_part_def, mk_ffi_next_def] >>
+      qmatch_goalsub_abbrev_tac`IO st f ns` >>
       CONV_TAC(RESORT_EXISTS_CONV List.rev) >>
-      map_every qexists_tac[`events`,`ns`,`f`,`st`] >>
+      map_every qexists_tac[`ns`,`f`] >>
       xsimpl >> qexists_tac`n2w8 fd` >>
       fs[Abbr`f`,Abbr`st`,Abbr`ns`,mk_ffi_next_def,
          ffi_read_def,w82n_n2w8,LENGTH_n2w8,MEM_MAP, ORD_BOUND,ORD_eq_0,wfFS_LDROP,
@@ -1655,13 +1412,10 @@ Proof
       cases_on`fs.numchars` >> fs[wfFS_def,liveFS_def,live_numchars_def] >>
       fs[n2w2_def,DIV_MOD_MOD_DIV,DIV_DIV_DIV_MULT] >> xsimpl >>
       qmatch_goalsub_abbrev_tac`(k DIV 256) MOD 256 = _ MOD 256` >> qexists_tac`k` >>
-      xsimpl >> fs[MIN_LE,eof_def,Abbr`k`,NUM_def,INT_def] >>
-      qpat_abbrev_tac `new_events = events ++ _` >>
-      qexists_tac `new_events` >> xsimpl) >>
+      xsimpl >> fs[MIN_LE,eof_def,Abbr`k`,NUM_def,INT_def]) >>
    rpt(xlet_auto >- xsimpl) >>
    xif >> instantiate >> xapp >> xsimpl >> rw[] >> instantiate >>
-   simp[GSYM n2w2_def,w22n_n2w2] >> xsimpl
-QED
+   simp[GSYM n2w2_def,w22n_n2w2] >> xsimpl);
 
 Theorem read_into_spec
   `!fs fd fdv n nv buf. wfFS fs ⇒ FD fd fdv ⇒ NUM n nv ⇒
@@ -1757,8 +1511,8 @@ Theorem read_into_spec
    xif >> instantiate >> xapp >> xsimpl >> rw[] >> instantiate >>
    simp[GSYM n2w2_def,w22n_n2w2] >> xsimpl);
 
-Theorem read_byte_spec:
-   !fd fdv content pos.
+Theorem read_byte_spec
+  `!fd fdv content pos.
     FD fd fdv ⇒
     get_file_content fs fd = SOME(content, pos) ⇒
     get_mode fs fd = SOME ReadMode ⇒
@@ -1769,9 +1523,8 @@ Theorem read_byte_spec:
             eof fd fs = SOME F) *
             IOFS (bumpFD fd fs 1))
       (\e.  &(EndOfFile_exn e /\ eof fd fs = SOME T) *
-            IOFS(bumpFD fd fs 0)))
-Proof
-  xcf_with_def "TextIO.read_byte" TextIO_read_byte_v_def >>
+            IOFS(bumpFD fd fs 0)))`
+  (xcf_with_def "TextIO.read_byte" TextIO_read_byte_v_def >>
   fs[IOFS_def,IOFS_iobuff_def] >>
   xpull >> rename [`W8ARRAY _ bdef`] >>
   Cases_on `bdef` >> fs[] >> qmatch_goalsub_rename_tac`h1 :: t` >>
@@ -1785,11 +1538,10 @@ Proof
          fs[EndOfFile_exn_def,eof_def,get_file_content_def,liveFS_bumpFD] >> xsimpl) >>
   xapp >> xsimpl >>
   `nr = 1` by fs[] >> fs[] >> xsimpl >>
-  fs[TAKE1_DROP,eof_def,get_file_content_def] >> pairarg_tac >> fs[liveFS_bumpFD]
-QED
+  fs[TAKE1_DROP,eof_def,get_file_content_def] >> pairarg_tac >> fs[liveFS_bumpFD]);
 
-Theorem read_byte_STDIO_spec:
-    FD fd fdv ∧ fd ≠ 1 ∧ fd ≠ 2 ∧
+Theorem read_byte_STDIO_spec
+  ` FD fd fdv ∧ fd ≠ 1 ∧ fd ≠ 2 ∧
     get_file_content fs fd = SOME(content, pos) ⇒
     get_mode fs fd = SOME ReadMode ⇒
     app (p:'ffi ffi_proj) TextIO_read_byte_v [fdv]
@@ -1799,20 +1551,18 @@ Theorem read_byte_STDIO_spec:
             eof fd fs = SOME F) *
             STDIO (bumpFD fd fs 1))
       (\e.  &(EndOfFile_exn e /\ eof fd fs = SOME T) *
-            STDIO(bumpFD fd fs 0)))
-Proof
-  rw[STDIO_def] >> xpull >> xapp_spec read_byte_spec >>
+            STDIO(bumpFD fd fs 0)))`
+  (rw[STDIO_def] >> xpull >> xapp_spec read_byte_spec >>
   mp_tac(GSYM(SPEC_ALL get_file_content_numchars)) >> rw[] >>
   mp_tac(get_mode_with_numchars) >> rw[] >>
   instantiate >> xsimpl >>
   simp[bumpFD_forwardFD,forwardFD_numchars,STD_streams_forwardFD] \\
-  rw[] \\ qexists_tac`THE (LTL ll)` \\ xsimpl
-QED
+  rw[] \\ qexists_tac`THE (LTL ll)` \\ xsimpl);
 
 (* TODO: call the low-level IOFS specs with the non-standard name, not vice versa *)
 
-Theorem input1_spec:
-    INSTREAM fd fdv ∧ fd ≠ 1 ∧ fd ≠ 2 ∧
+Theorem input1_spec
+  ` INSTREAM fd fdv ∧ fd ≠ 1 ∧ fd ≠ 2 ∧
     get_file_content fs fd = SOME(content, pos) ⇒
     get_mode fs fd = SOME ReadMode ⇒
     app (p:'ffi ffi_proj) TextIO_input1_v [fdv]
@@ -1825,9 +1575,8 @@ Theorem input1_spec:
       | SOME T =>
         &OPTION_TYPE CHAR NONE v *
         STDIO (bumpFD fd fs 0)
-      | _ => &F)
-Proof
-  xcf_with_def "TextIO.input1" TextIO_input1_v_def
+      | _ => &F)`
+  (xcf_with_def "TextIO.input1" TextIO_input1_v_def
   \\ xhandle`POSTve (λv. &OPTION_TYPE CHAR (SOME (EL pos content)) v *
                          STDIO (forwardFD fs fd 1) * &(eof fd fs = SOME F))
                     (λe. &EndOfFile_exn e * STDIO fs * &(eof fd fs = SOME T))`
@@ -1847,11 +1596,10 @@ Proof
   \\ reverse conj_tac >- (EVAL_TAC \\ fs[])
   \\ xcon
   \\ xsimpl
-  \\ fs[std_preludeTheory.OPTION_TYPE_def]
-QED
+  \\ fs[std_preludeTheory.OPTION_TYPE_def]);
 
-Theorem input_IOFS_spec:
-   !fd fdv fs content pos off offv.
+Theorem input_IOFS_spec
+  `!fd fdv fs content pos off offv.
     len + off <= LENGTH buf ∧
     INSTREAM fd fdv ∧ NUM off offv ∧ NUM len lenv ∧
     get_file_content fs fd = SOME(content, pos) ⇒
@@ -1861,9 +1609,8 @@ Theorem input_IOFS_spec:
     (POSTv nv. &(NUM (MIN len (LENGTH content - pos)) nv) *
        W8ARRAY bufv (insert_atI (TAKE len (DROP pos (MAP (n2w o ORD) content)))
                                  off buf) *
-       SEP_EXISTS k. IOFS (fsupdate fs fd k (MIN (len + pos) (MAX pos (LENGTH content))) content))
-Proof
-  xcf_with_def "TextIO.input" TextIO_input_v_def >>
+       SEP_EXISTS k. IOFS (fsupdate fs fd k (MIN (len + pos) (MAX pos (LENGTH content))) content))`
+  (xcf_with_def "TextIO.input" TextIO_input_v_def >>
   reverse(Cases_on`pos ≤ LENGTH content`) >- (
     imp_res_tac get_file_content_eof \\ rfs[] \\
     reverse(Cases_on`wfFS fs`) >- (fs[IOFS_def] \\ xpull) \\
@@ -1909,7 +1656,7 @@ Proof
     \\ qmatch_abbrev_tac`IOFS f1 ==>> IOFS f2 * _`
     \\ `f1 = f2` by (
       simp[Abbr`f1`,Abbr`f2`,IO_fs_component_equality]
-      \\ simp[AFUPDKEY_unchanged] )
+      \\ simp[ALIST_FUPDKEY_unchanged] )
     \\ xsimpl )
   \\ `MAX pos (LENGTH content) = LENGTH content` by rw[MAX_DEF]
   \\ pop_assum SUBST_ALL_TAC >>
@@ -1946,14 +1693,13 @@ Proof
      qexists_tac `1` >>
      fs[get_file_content_def] >> pairarg_tac >> rw[] >>
      fs[wfFS_fsupdate,liveFS_fsupdate,MIN_DEF,MEM_MAP,insert_atI_NIL,
-        validFD_ALOOKUP, bumpFD_def, fsupdate_def,LDROP_1,consistentFS_def,
-        AFUPDKEY_unchanged,wfFS_def,liveFS_def,live_numchars_def]
-     >-(metis_tac[]) >>
+        validFD_ALOOKUP, bumpFD_def, fsupdate_def,LDROP_1,
+        ALIST_FUPDKEY_unchanged,wfFS_def,liveFS_def,live_numchars_def] >>
      cases_on`fs'.numchars` >> fs[LDROP_1,NOT_LFINITE_DROP_LFINITE] >>
      cases_on`fs'.numchars` >> fs[LDROP_1] >> cases_on`fs` >>
      qmatch_abbrev_tac`IOx _ fs1 ==>> IOx _ fs2 * GC` >>
      `fs1 = fs2` by (unabbrev_all_tac >>
-                     fs[IO_fs_component_equality,AFUPDKEY_unchanged]) >>
+                     fs[IO_fs_component_equality,ALIST_FUPDKEY_unchanged]) >>
      xsimpl) >>
   last_x_assum xapp_spec>> fs[IOFS_def,IOFS_iobuff_def] >> xpull >>
   rw[] >> cases_on`len'`
@@ -1972,14 +1718,13 @@ Proof
      qexists_tac `1` >>
      fs[get_file_content_def] >> pairarg_tac >> rw[] >>
      fs[wfFS_fsupdate,liveFS_fsupdate,MIN_DEF,MEM_MAP,insert_atI_NIL,
-        validFD_ALOOKUP, bumpFD_def, fsupdate_def,LDROP_1,consistentFS_def,
-        AFUPDKEY_unchanged,wfFS_def,liveFS_def,live_numchars_def]
-     >-(metis_tac[]) >>
+        validFD_ALOOKUP, bumpFD_def, fsupdate_def,LDROP_1,
+        ALIST_FUPDKEY_unchanged,wfFS_def,liveFS_def,live_numchars_def] >>
      cases_on`fs'.numchars` >> fs[LDROP_1,NOT_LFINITE_DROP_LFINITE] >>
      cases_on`fs'.numchars` >> fs[LDROP_1] >> cases_on`fs` >>
      qmatch_abbrev_tac`IOx _ fs1 ==>> IOx _ fs2 * GC` >>
      `fs1 = fs2` suffices_by xsimpl >>
-     unabbrev_all_tac >> fs[IO_fs_component_equality,AFUPDKEY_unchanged]) >>
+     unabbrev_all_tac >> fs[IO_fs_component_equality,ALIST_FUPDKEY_unchanged]) >>
   xlet_auto >- xsimpl >>
   rename [`W8ARRAY iobuff_loc bdef`] >>
   Cases_on `bdef` >> fs[] >> qmatch_goalsub_rename_tac`h1::t` >>
@@ -1995,19 +1740,19 @@ Proof
   xlet_auto >- xsimpl >>
   `MEM fd (MAP FST fs'.infds)` by
      (fs[get_file_content_def] >> pairarg_tac >> fs[ALOOKUP_MEM,MEM_MAP] >>
-      qexists_tac`fd,(ino, md,pos'')` >> fs[ALOOKUP_MEM]) >>
+      qexists_tac`fd,(fnm, md,pos'')` >> fs[ALOOKUP_MEM]) >>
   xif
   >-(xvar >> xsimpl >> qexists_tac`1` >>
      fs[eof_def] >> pairarg_tac >> fs[get_file_content_def] >>
      pairarg_tac \\ fs[] \\ rveq \\
      `LENGTH content = pos'` by (fs[] >> rfs[]) >>
-     fs[MIN_DEF,liveFS_fsupdate,insert_atI_NIL,bumpFD_def,AFUPDKEY_unchanged] >>
+     fs[MIN_DEF,liveFS_fsupdate,insert_atI_NIL,bumpFD_def,ALIST_FUPDKEY_unchanged] >>
      rw[DROP_NIL] >- fs[validFD_def,wfFS_fsupdate]
      >- fs[GSYM MAP_DROP,DROP_LENGTH_NIL,insert_atI_NIL] >>
      qmatch_abbrev_tac `IOx _ fs1 ==>> IOx _ fs2 * GC` >>
      `fs1 = fs2` suffices_by xsimpl >>
      unabbrev_all_tac >> cases_on`fs'.numchars` >>
-     fs[IO_fs_component_equality,AFUPDKEY_unchanged,fsupdate_def,LDROP_1,
+     fs[IO_fs_component_equality,ALIST_FUPDKEY_unchanged,fsupdate_def,LDROP_1,
         wfFS_def,liveFS_def,live_numchars_def]) >>
   NTAC 4 (xlet_auto >- xsimpl) >>
   qmatch_goalsub_abbrev_tac`W8ARRAY bufv buf'' * W8ARRAY iobuff_loc _ *
@@ -2019,7 +1764,7 @@ Proof
   fs[get_file_content_def, validFD_bumpFD,liveFS_bumpFD,bumpFD_def,get_mode_def] >>
   xsimpl >>
   fs[get_file_content_def, validFD_bumpFD,liveFS_bumpFD,bumpFD_def,get_mode_def,
-     AFUPDKEY_ALOOKUP,INT_OF_NUM_SUBS_2,NUM_def,INT_def] >>
+     ALIST_FUPDKEY_ALOOKUP,INT_OF_NUM_SUBS_2,NUM_def,INT_def] >>
   rw[] >> qexists_tac`SUC x''` >>
   fs[NUM_def,INT_def,MIN_DEF,validFD_def,wfFS_fsupdate,liveFS_fsupdate] >>
   strip_tac
@@ -2035,14 +1780,13 @@ Proof
   `fs1 = fs2` suffices_by xsimpl >>
   unabbrev_all_tac >> cases_on`fs'.numchars` >> fs[wfFS_def,liveFS_def,live_numchars_def] >>
   pairarg_tac \\
-  fs[IO_fs_component_equality,AFUPDKEY_unchanged,fsupdate_def,LDROP_1] >>
-  fs[AFUPDKEY_ALOOKUP,AFUPDKEY_o,AFUPDKEY_eq] >>
-  simp[AFUPDKEY_unchanged])
-  \\ xapp \\ instantiate \\ xsimpl
-QED
+  fs[IO_fs_component_equality,ALIST_FUPDKEY_unchanged,fsupdate_def,LDROP_1] >>
+  fs[ALIST_FUPDKEY_ALOOKUP,ALIST_FUPDKEY_o,ALIST_FUPDKEY_eq] >>
+  simp[ALIST_FUPDKEY_unchanged])
+  \\ xapp \\ instantiate \\ xsimpl);
 
-Theorem input_spec:
-   !fd fdv fs content pos off offv len lenv buf bufv.
+Theorem input_spec
+  `!fd fdv fs content pos off offv len lenv buf bufv.
     len + off <= LENGTH buf ∧
     INSTREAM fd fdv ∧ NUM off offv ∧ NUM len lenv ∧
     get_file_content fs fd = SOME(content, pos) ⇒
@@ -2054,9 +1798,8 @@ Theorem input_spec:
                                  off buf)) *
        W8ARRAY bufv (insert_atI (TAKE len (DROP pos (MAP (n2w o ORD) content)))
                                  off buf) *
-        STDIO (fsupdate fs fd 0 (MIN (len + pos) (MAX pos (LENGTH content))) content))
-Proof
-  rw[STDIO_def]
+        STDIO (fsupdate fs fd 0 (MIN (len + pos) (MAX pos (LENGTH content))) content))`
+  (rw[STDIO_def]
   \\ xpull
   \\ `fd = 1 ∨ fd = 2 ⇒ pos = LENGTH content`
   by (
@@ -4742,27 +4485,24 @@ Theorem b_inputLines_spec
       >-(cheat))
     >-(cheat)));
 
-Theorem extend_array_spec:
-     ∀arrv arr.
+Theorem extend_array_spec
+    `∀arrv arr.
      app (p:'ffi ffi_proj) TextIO_extend_array_v [arrv] (W8ARRAY arrv arr)
-       (POSTv v. W8ARRAY v (arr ++ (REPLICATE (LENGTH arr) 0w)))
-Proof
-    xcf_with_def "TextIO.extend_array" TextIO_extend_array_v_def
+        (POSTv v. W8ARRAY v (arr ++ (REPLICATE (LENGTH arr) 0w)))`
+    (xcf_with_def "TextIO.extend_array" TextIO_extend_array_v_def
     \\ ntac 5 (xlet_auto >- xsimpl)
     \\ xret \\ xsimpl
-    \\ simp[DROP_REPLICATE]
-QED
+    \\ simp[DROP_REPLICATE] );
 
-Theorem inputLine_spec:
-   INSTREAM fd fdv ∧ IS_SOME (get_file_content fs fd) ∧ get_mode fs fd = SOME ReadMode
+Theorem inputLine_spec
+  `INSTREAM fd fdv ∧ IS_SOME (get_file_content fs fd) ∧ get_mode fs fd = SOME ReadMode
    ⇒
    app (p:'ffi ffi_proj) TextIO_inputLine_v [fdv]
      (STDIO fs)
      (POSTv sov.
        &OPTION_TYPE STRING_TYPE (OPTION_MAP implode (lineFD fs fd)) sov *
-       STDIO (lineForwardFD fs fd))
-Proof
-  strip_tac \\
+       STDIO (lineForwardFD fs fd))`
+  (strip_tac \\
   xcf_with_def "TextIO.inputLine" TextIO_inputLine_v_def \\
   xlet_auto >- xsimpl \\
   xlet_auto >- xsimpl \\
@@ -5028,11 +4768,10 @@ Proof
   \\ qexists_tac`pos` \\ simp[]
   \\ instantiate
   \\ xsimpl
-  \\ EVAL_TAC
-QED
+  \\ EVAL_TAC);
 
-Theorem inputLines_spec:
-   !fd fdv fs. INSTREAM fd fdv ∧
+Theorem inputLines_spec
+  `!fd fdv fs. INSTREAM fd fdv ∧
    get_file_content fs fd = SOME (content,pos) ∧
    get_mode fs fd = SOME ReadMode
    ⇒
@@ -5042,9 +4781,8 @@ Theorem inputLines_spec:
        &LIST_TYPE STRING_TYPE
          (MAP (\x. strcat (implode x) (implode "\n"))
             (splitlines (DROP pos content))) fcv *
-       STDIO (fastForwardFD fs fd))
-Proof
-  Induct_on`splitlines (DROP pos content)` \\ rw[]
+       STDIO (fastForwardFD fs fd))`
+  (Induct_on`splitlines (DROP pos content)` \\ rw[]
   >- (
     qpat_x_assum`[] = _`(assume_tac o SYM) \\ fs[DROP_NIL]
     \\ `LENGTH content - pos = 0` by simp[]
@@ -5100,28 +4838,26 @@ Proof
   \\ Cases_on`LENGTH h = LENGTH content - pos` \\ fs[]
   \\ imp_res_tac SPLITP_JOIN
   \\ pop_assum(mp_tac o Q.AP_TERM`LENGTH`) \\ simp[]
-  \\ Cases_on`LENGTH r = 0` \\ simp[] \\ fs[]
-QED
+  \\ Cases_on`LENGTH r = 0` \\ simp[] \\ fs[] );
 
-Theorem inputLinesFrom_spec:
-   FILENAME f fv /\ hasFreeFD fs
+Theorem inputLinesFrom_spec
+  `FILENAME f fv /\ hasFreeFD fs
    ⇒
    app (p:'ffi ffi_proj) TextIO_inputLinesFrom_v
      [fv]
      (STDIO fs)
      (POSTv sv. &OPTION_TYPE (LIST_TYPE STRING_TYPE)
-            (if inFS_fname fs f then
-               SOME(all_lines fs f)
+            (if inFS_fname fs (File f) then
+               SOME(all_lines fs (File f))
              else NONE) sv
-             * STDIO fs)
-Proof
-  xcf_with_def "TextIO.inputLinesFrom" TextIO_inputLinesFrom_v_def
+             * STDIO fs)`
+  (xcf_with_def "TextIO.inputLinesFrom" TextIO_inputLinesFrom_v_def
   \\ reverse(xhandle`POSTve
        (λv. &OPTION_TYPE (LIST_TYPE STRING_TYPE)
-         (if inFS_fname fs f
-          then SOME(all_lines fs f)
+         (if inFS_fname fs (File f)
+          then SOME(all_lines fs (File f))
           else NONE) v * STDIO fs)
-       (λe. &(BadFileName_exn e ∧ ¬inFS_fname fs f) * STDIO fs)`)
+       (λe. &(BadFileName_exn e ∧ ¬inFS_fname fs (File f)) * STDIO fs)`)
   >- (xcases \\ fs[BadFileName_exn_def]
       \\ reverse conj_tac >- (EVAL_TAC \\ rw[])
       \\ xcon \\ xsimpl \\ fs[std_preludeTheory.OPTION_TYPE_def])
@@ -5129,9 +4865,6 @@ Proof
   \\ `CARD (set (MAP FST fs.infds)) < fs.maxFD` by fs[]
   \\ reverse(Cases_on`STD_streams fs`)
   >- ( fs[STDIO_def] \\ xpull )
-  \\ reverse(Cases_on`consistentFS fs`)
-  >- (fs[STDIO_def,IOFS_def,wfFS_def] \\ xpull
-      \\ fs[consistentFS_def] \\ res_tac)
   \\ xlet_auto_spec (SOME (SPEC_ALL openIn_STDIO_spec))
   >- (
     xsimpl
@@ -5142,17 +4875,16 @@ Proof
     xsimpl
     \\ rw[inFS_fname_numchars]
     \\ qexists_tac`ll` \\ xsimpl )
+  \\ drule (GEN_ALL ALOOKUP_inFS_fname_openFileFS_nextFD)
   \\ imp_res_tac nextFD_ltX
-  \\ progress inFS_fname_ALOOKUP_EXISTS
-  \\ progress ALOOKUP_inFS_fname_openFileFS_nextFD
-  \\ rfs[]
-  \\ pop_assum(qspec_then`0`strip_assume_tac)
+  \\ disch_then(qspec_then`0`mp_tac) \\ rw[]
   \\ qmatch_assum_abbrev_tac`validFD fd fso`
-  \\ imp_res_tac inFS_fname_ALOOKUP_EXISTS \\ res_tac
   \\ `∃c. get_file_content fso fd = SOME (c,0)`
-    by (fs[get_file_content_def,validFD_def,Abbr`fso`,openFileFS_inode_tbl])
+  by (
+    fs[get_file_content_def,validFD_def,Abbr`fso`,openFileFS_files]
+    \\ imp_res_tac inFS_fname_ALOOKUP_EXISTS \\ fs[] )
   \\ `get_mode fso fd = SOME ReadMode`
-  by ( fs[Abbr`fso`, openFileFS_def, get_mode_def,get_file_content_fsupdate] )
+  by ( simp[Abbr`fso`, openFileFS_def, get_mode_def] )
   \\ xlet_auto >- xsimpl
   \\ qmatch_goalsub_abbrev_tac`STDIO fsob`
   \\ rename1 `INSTREAM fd fdv`
@@ -5183,52 +4915,51 @@ Proof
   \\ fs[all_lines_def,lines_of_def]
   \\ fs[get_file_content_def]
   \\ pairarg_tac \\ fs[]
-  \\ fs[Abbr`fso`,openFileFS_inode_tbl]
+  \\ fs[Abbr`fso`,openFileFS_files]
   \\ rveq \\ fs[]
   \\ qmatch_goalsub_abbrev_tac`STDIO fs'`
   \\ first_x_assum(qspec_then`ReadMode`mp_tac) \\ strip_tac \\ fs[]
   \\ `fs' = fs` suffices_by ( rw[std_preludeTheory.OPTION_TYPE_def] \\ xsimpl)
   \\ unabbrev_all_tac
-  \\ simp[fastForwardFD_def,ADELKEY_AFUPDKEY,o_DEF,
-          libTheory.the_def, openFileFS_numchars,openFileFS_files,
-          IO_fs_component_equality,openFileFS_inode_tbl]
-QED
+  \\ simp[fastForwardFD_def,A_DELKEY_ALIST_FUPDKEY,o_DEF,
+          libTheory.the_def, openFileFS_numchars,
+          IO_fs_component_equality,openFileFS_files]);
 
 val inputLinesFrom_def = Define `
   inputLinesFrom f =
-    (\fs. (Success (if inFS_fname fs f then
-                      SOME(all_lines fs f)
+    (\fs. (Success (if inFS_fname fs (File f) then
+                      SOME(all_lines fs (File f))
                     else NONE), fs))`;
 
-Theorem EvalM_inputLinesFrom:
-   Eval env exp (FILENAME f) /\
+Theorem EvalM_inputLinesFrom
+  `Eval env exp (FILENAME f) /\
     (nsLookup env.v (Long "TextIO" (Short "inputLinesFrom")) =
        SOME TextIO_inputLinesFrom_v) ==>
     EvalM F env st (App Opapp [Var (Long "TextIO" (Short "inputLinesFrom")); exp])
       (MONAD (OPTION_TYPE (LIST_TYPE STRING_TYPE)) exc_ty (inputLinesFrom f))
-      (MONAD_IO,p:'ffi ffi_proj)
-Proof
-  ho_match_mp_tac EvalM_from_app
-    \\ rw[inputLinesFrom_def]
-    \\ rw[MONAD_IO_def]
-    \\ xpull
-    \\ fs[SEP_CLAUSES]
-    \\ xapp_spec inputLinesFrom_spec
-    \\ fs[]
-    \\ rpt (xsimpl \\ asm_exists_tac)
-QED
+      (MONAD_IO,p:'ffi ffi_proj)`
+  (ho_match_mp_tac EvalM_from_app
+  \\ conj_tac >- rw [inputLinesFrom_def]
+  \\ rw [MONAD_IO_def]
+  \\ xpull
+  \\ fs [SEP_CLAUSES]
+  \\ match_mp_tac (app_weaken |> SIMP_RULE (srw_ss()) [AND_IMP_INTRO])
+  \\ drule (GEN_ALL inputLinesFrom_spec)
+  \\ disch_then (qspecl_then [`p`,`s`] assume_tac)
+  \\ rfs [inputLinesFrom_def]
+  \\ asm_exists_tac \\ fs []
+  \\ xsimpl);
 
-Theorem inputAll_spec:
-   INSTREAM fd fdv ∧
+Theorem inputAll_spec
+  `INSTREAM fd fdv ∧
    get_file_content fs fd = SOME (content,pos) ⇒
    get_mode fs fd = SOME ReadMode ⇒
    app (p:'ffi ffi_proj) TextIO_inputAll_v [fdv]
    (STDIO fs)
    (POSTv v.
      &STRING_TYPE (implode (DROP pos content)) v *
-     STDIO (fastForwardFD fs fd))
-Proof
-  xcf_with_def "TextIO.inputAll" TextIO_inputAll_v_def \\
+     STDIO (fastForwardFD fs fd))`
+  (xcf_with_def "TextIO.inputAll" TextIO_inputAll_v_def \\
   reverse(Cases_on`pos ≤ LENGTH content`)
   >- (
     xfun_spec `inputAll_aux`
@@ -5336,7 +5067,7 @@ Proof
         simp[Abbr`fs2`,forwardFD_def,fsupdate_def]
         \\ fs[get_file_content_def]
         \\ rpt (pairarg_tac \\ fs[])
-        \\ fs[IO_fs_component_equality,AFUPDKEY_unchanged,AFUPDKEY_eq] )
+        \\ fs[IO_fs_component_equality,ALIST_FUPDKEY_unchanged,ALIST_FUPDKEY_eq] )
       \\ qunabbrev_tac`fs2` \\ pop_assum SUBST_ALL_TAC
       \\ simp[fastForwardFD_forwardFD]
       \\ xsimpl
@@ -5364,16 +5095,14 @@ Proof
   \\ disch_then(first_assum o mp_then Any mp_tac)
   \\ simp[Abbr`arrmax`,MAX_DEF,Once REPLICATE_compute]
   \\ strip_tac
-  \\ xapp \\ xsimpl
-QED
+  \\ xapp \\ xsimpl );
 
-Theorem print_list_spec:
-   ∀ls lv fs out. LIST_TYPE STRING_TYPE ls lv ⇒
+Theorem print_list_spec
+  `∀ls lv fs out. LIST_TYPE STRING_TYPE ls lv ⇒
    app (p:'ffi ffi_proj) TextIO_print_list_v [lv]
      (STDIO fs)
-     (POSTv v. &UNIT_TYPE () v * STDIO (add_stdout fs (concat ls)))
-Proof
-  Induct \\ rw[LIST_TYPE_def]
+     (POSTv v. &UNIT_TYPE () v * STDIO (add_stdout fs (concat ls)))`
+  (Induct \\ rw[LIST_TYPE_def]
   \\ xcf_with_def "TextIO.print_list" TextIO_print_list_v_def
   \\ (reverse(Cases_on`STD_streams fs`) >- (fs[STDIO_def] \\ xpull))
   \\ xmatch
@@ -5385,121 +5114,6 @@ Proof
   \\ imp_res_tac add_stdo_o
   \\ simp[concat_cons]
   \\ map_every qexists_tac [`emp`,`add_stdout fs s`]
-  \\ xsimpl
-QED
-
-(* input and output file descriptors need to bind to different inodes to ensure termination *)
-Theorem copy_spec:
-   ∀ ino1 ino2 content1 inp out pos content2 fs inpv outv.
-      INSTREAM inp inpv /\ OUTSTREAM out outv /\ ino1 <> ino2 /\
-      ALOOKUP fs.infds inp = SOME (ino1,ReadMode,pos) /\
-      ALOOKUP fs.infds out = SOME (ino2,WriteMode,LENGTH content2) /\
-      ALOOKUP fs.inode_tbl ino1 = SOME content1 /\
-      ALOOKUP fs.inode_tbl ino2 = SOME content2 /\
-      pos <= STRLEN content1 ⇒
-      app (p:'ffi ffi_proj) TextIO_copy_v [inpv;outv]
-       (STDIO fs)
-       (POSTv u. &UNIT_TYPE () u *
-              STDIO (fsupdate (fastForwardFD fs inp)
-                              out 0
-                              (LENGTH content2 + (LENGTH content1) - pos)
-                              (content2 ++ (DROP pos content1))))
-Proof
-  NTAC 6 strip_tac >>
-  `?N. STRLEN content1 - pos <= N`
-    by (qexists_tac`STRLEN content1 - pos` >> fs[]) >>
-  FIRST_X_ASSUM MP_TAC >> qid_spec_tac`pos` >>
-  Induct_on`N` >> rw[] >>
-  xcf_with_def "TextIO.copy" TextIO_copy_v_def >>
-  fs[STDIO_def,IOFS_def,IOFS_iobuff_def] >> xpull >>
-  rename [`W8ARRAY _ bdef`] >>
-  Cases_on `bdef` >> fs[] >> qmatch_goalsub_rename_tac`h1::t` >>
-  Cases_on `t` >> fs[] >> qmatch_goalsub_abbrev_tac`h1::h2::t` >>
-  Cases_on `t` >> fs[] >> qmatch_goalsub_abbrev_tac`h1::h2::h3::t` >>
-  Cases_on `t` >> fs[] >> qmatch_goalsub_abbrev_tac`h1::h2::h3::h4::t` >>
-  PURE_REWRITE_TAC[GSYM iobuff_loc_def] >>
-  `inp <> out` by (strip_tac >> fs[]) >>
-  (fs[INSTREAM_def] >> xlet_auto >- xsimpl >> fs[get_in_def] >>
-  xlet_auto_spec (SOME (Q.SPECL[`fs with numchars := ll`,`inp`] read_spec))
-   >-(rw[FD_def,get_file_content_def] >> xsimpl >> rw[]  >> instantiate  >> xsimpl)
-   >-(rw[get_file_content_def,get_mode_def] >> xsimpl)
-   >>(rw[get_file_content_def] >> xsimpl) >>
-   xlet_auto >- xsimpl) >>
-  (xif
-    >-(xcon >>
-       fs[eof_def] >> pairarg_tac >> fs[] >> rfs[] >> rw[] >>
-       `pos >= LENGTH content1` by fs[]  >> imp_res_tac DROP_NIL >> xsimpl >>
-       `get_file_content fs inp = SOME(content1,pos)`
-       by (fs[get_file_content_def] >> pairarg_tac >> fs[] >> rfs[]) >>
-       `get_file_content fs out = SOME(content2,LENGTH content2)`
-       by (fs[get_file_content_def] >> pairarg_tac >> fs[]) >>
-       fs[fastForwardFD_0,fsupdate_unchanged,bumpFD_0] >>
-       qexists_tac`THE (LTL ll)` >> xsimpl >> fs[wfFS_LTL]))
-   >-(fs[GSYM get_file_content_numchars] >>
-      `get_file_content fs inp = SOME(content1,pos)`
-     by (fs[get_file_content_def] >> pairarg_tac >> fs[] >> rfs[]) >> fs[]) >>
-   fs[OUTSTREAM_def] >> xlet_auto >- xsimpl >> fs[get_out_def] >>
-   `content = content1 /\ pos' = pos`
-     by (fs[GSYM get_file_content_numchars,get_file_content_def] >>
-         rfs[] >> pairarg_tac >> rw[] >> fs[]) >>
-   NTAC 2 (first_x_assum (fn x => fs [x])) >>
-   qmatch_goalsub_abbrev_tac`IOx _ fs'` >>
-   `get_file_content fs' out = SOME(content2,LENGTH content2)`
-     by (fs[get_file_content_def,Abbr`fs'`,bumpFD_def,AFUPDKEY_ALOOKUP]) >>
-   xlet_auto
-   >-(fs[FD_def,iobuff_loc_def,Abbr`fs'`,liveFS_bumpFD,liveFS_def,validFD_bumpFD,
-         validFD_numchars,ALOOKUP_validFD,get_mode_def] >> xsimpl) >>
-   fs[MAP_MAP_o, CHR_w2n_n2w_ORD,TAKE_APPEND1,TAKE_TAKE,insert_atI_end] >>
-   qmatch_goalsub_abbrev_tac`IOFS fs''` >>
-   xapp >> fs[IOFS_def,IOFS_iobuff_def] >> xsimpl >>
-   fs[AFUPDKEY_ALOOKUP,insert_atI_def] >>
-   map_every qexists_tac [`emp`, `pos + nr`,`fs''`,`content2 ++ TAKE nr (DROP pos content1)`] >>
-   xsimpl >> rw[Abbr`fs''`, Abbr`fs'`]
-   >-(fs[fsupdate_def,AFUPDKEY_ALOOKUP,bumpFD_def])
-   >-(fs[fsupdate_def,AFUPDKEY_ALOOKUP,bumpFD_def])
-   >-(fs[fsupdate_def,AFUPDKEY_ALOOKUP,bumpFD_def])
-   >-(fs[fsupdate_def,AFUPDKEY_ALOOKUP,bumpFD_def])
-   >-(qexists_tac`THE (LDROP k (THE (LTL ll)))` >> rw[]
-      >-(fs[fsupdate_numchars] >> irule wfFS_fsupdate >> conj_tac
-         >-(
-            `(bumpFD inp (fs with numchars := ll) nr).numchars = THE (LTL ll)`
-               by fs[bumpFD_numchars] >>
-             first_x_assum (fn x => rw[GSYM x]) >>
-            fs[wfFS_bumpFD,wfFS_LDROP ])
-         >-(fs[bumpFD_def,MAP_FST_AFUPDKEY] >> simp[MEM_MAP] >>
-            imp_res_tac ALOOKUP_MEM >>
-            qexists_tac`(out,ino2,WriteMode,STRLEN content2)` >> fs[]))
-      >-(irule STD_streams_fsupdate >> rw[] >>
-         `inp <> 1 /\ inp <> 2` by (
-           fs[STD_streams_def] >>
-           first_x_assum(assume_tac o Q.SPECL [`inp`,`WriteMode`,`STRLEN err`]) >>
-           first_x_assum(assume_tac o Q.SPECL [`inp`,`WriteMode`,`STRLEN out'`]) >>
-           rfs[]) >>
-         fs[GEN_ALL STD_streams_bumpFD,GSYM STD_streams_numchars])
-      >-(qmatch_abbrev_tac`IOx fs_ffi_part fs1 ==>> IOx fs_ffi_part fs2` >>
-         `fs2 = fs1` suffices_by xsimpl >> unabbrev_all_tac >>
-         fs[AFUPDKEY_ALOOKUP,insert_atI_end,TAKE_APPEND,TAKE_TAKE, fsupdate_def,
-            bumpFD_def,AFUPDKEY_unchanged] >> rw[IO_fs_component_equality]))
-   >-(qexists_tac`x` >>
-      qmatch_goalsub_abbrev_tac`IOx fs_ffi_part (fs1 with numchars := x)
-                           ==>> IOx fs_ffi_part (fs2 with numchars := x) * GC` >>
-      fs[bumpFD_forwardFD,fsupdate_numchars,fastForwardFD_with_numchars] >>
-      `fs1 with numchars := x = fs2 with numchars := x` by (
-         unabbrev_all_tac >>
-         qmatch_goalsub_abbrev_tac`fsupdate fs' out k _ _` >>
-         `ALOOKUP fs'.infds inp = SOME (ino1,ReadMode,nr + pos) ∧
-          ALOOKUP fs'.infds out = SOME (ino2,WriteMode,STRLEN content2) ∧
-          ALOOKUP fs'.inode_tbl ino1 = SOME content1 ∧
-          ALOOKUP fs'.inode_tbl ino2 = SOME content2`
-           by fs[Abbr`fs'`,forwardFD_def,AFUPDKEY_ALOOKUP] >>
-         fs[GSYM fsupdate_fastForwardFD_comm,fsupdate_numchars] >>
-         fs[Abbr`fs'`,fastForwardFD_with_numchars,fastForwardFD_forwardFD] >>
-         fs[GSYM DROP_DROP] >>
-         PURE_REWRITE_TAC[Once (GSYM STRCAT_ASSOC),TAKE_DROP] >> simp[]) >>
-         xsimpl >> fs[] >>
-         first_x_assum (fn z => PURE_REWRITE_TAC
-            [Once (Q.SPECL [`fs`,`x`] STD_streams_numchars),GSYM z]) >>
-         fs[GSYM STD_streams_numchars])
-QED
+  \\ xsimpl);
 
 val _ = export_theory();
